Lambda.v
@@ -7,9 +7,9 @@
 ********************************************************************************************)
 
 Set Implicit Arguments.
-Require Import Metatheory LambdaES_Defs LambdaES_Infra LambdaES_FV.
-Require Import Rewriting_Defs Rewriting_Lib.
-Require Import List.
+Require Import Metatheory LambdaES_Defs.
+Require Import Rewriting LambdaES_Infra LambdaES_FV.
+Require Import Arith List.
 
 (** The beta rule of the lambda calculus. **)
 Inductive rule_beta : pterm -> pterm -> Prop :=
@@ -25,9 +25,73 @@ Notation "t -->Beta+ u" := (Beta_trs t u) (at level 66).
 Definition Beta_str t u := star_closure Beta t u.
 Notation "t -->Beta* u" := (Beta_str t u) (at level 66).
 
-(* ********************************************************************** *)
-(** Properties of the  beta relation **)
 
+(* ********************************************************************** *)
+(** Properties of the  beta reduction **)
+
+Lemma Lterm_is_term: forall t, Lterm t -> term t.
+Proof.
+ intros. induction H; trivial.
+ apply term_distribute_over_application; split; trivial.
+ apply body_to_term_abs; trivial. unfold body.
+ exists L; trivial.
+Qed.
+
+Lemma Lbody_is_body: forall t, Lbody t -> body t.
+Proof.
+ intros. unfold body. unfold Lbody in H.
+ case H; clear H; intros L H. exists L.
+ intros x H'. apply Lterm_is_term.
+ apply H; trivial.
+Qed.
+
+Lemma subst_Lterm : forall t z u,
+  Lterm u -> Lterm t -> Lterm ([z ~> u]t).
+Proof.
+  induction 2; simpls*.
+  case_var*. apply_fresh Lterm_abs. rewrite* subst_open_var. apply Lterm_is_term; trivial.
+Qed.
+Hint Resolve subst_Lterm.
+
+Lemma Lbody_open_term : forall t u, Lbody t -> Lterm u -> Lterm (t ^^ u).
+Proof.
+ intros. destruct H. case var_fresh with (L := x \u (fv t)).
+ intros y Fr. rewrite* (@subst_intro y).
+Qed.
+
+Lemma not_Lbody_Sn: forall n, ~(Lbody (pterm_bvar (S n))).
+Proof.
+  intro n.
+  intro H. 
+  elim H.
+  intro L.
+  intro H1.
+  pick_fresh z.
+  assert (z \notin L). auto.
+  assert (Lterm (pterm_bvar (S n) ^ z)).
+  apply H1.
+  assumption.
+  inversion H2.
+Qed.
+
+(* ********************************************************************** *)
+(** Properties of reduction *)
+Definition L_red_regular (R : pterm -> pterm -> Prop) :=
+  forall t t', R t t' -> Lterm t /\ Lterm t'.
+
+Definition L_red_regular' (R : pterm -> pterm -> Prop) :=
+  forall t t', R t t' -> (Lterm t <-> Lterm t').
+
+Definition L_red_refl (R : pterm -> pterm -> Prop) :=
+  forall t, Lterm t -> R t t.
+
+Definition L_red_in (R : pterm -> pterm -> Prop) :=
+  forall t x u u', Lterm t -> R u u' ->
+  R ([x ~> u]t) ([x ~> u']t).
+
+Definition L_red_out (R : pterm -> pterm -> Prop) :=
+  forall x u t t', Lterm u -> R t t' -> 
+  R ([x~>u]t) ([x~>u]t').
 
 Lemma L_beta_regular : L_red_regular rule_beta.
 Proof. 
@@ -51,6 +115,14 @@ Proof.
  apply subst_Lterm; trivial. 
 Qed.
 
+Lemma L_red_out_to_rename : forall (R : pterm -> pterm -> Prop),
+  L_red_out R -> red_rename R. 
+Proof.
+  intros_all.
+  rewrite* (@subst_intro x t). 
+  rewrite* (@subst_intro x t').
+Qed.
+
 
 Lemma beta_rename : red_rename rule_beta.
 Proof.
@@ -58,7 +130,268 @@ Proof.
  apply L_beta_red_out.
 Qed.
 
+Lemma red_regular_Lctx : forall (R : pterm -> pterm -> Prop),
+  L_red_regular R -> L_red_regular (L_contextual_closure R).
+Proof. (*aqui*)
+  intros_all. induction H0.
+  apply H; trivial. 
+  case IHL_contextual_closure.
+  intros H2 H3.
+  split; apply Lterm_app; trivial. split; apply Lterm_app; trivial.
+  apply IHL_contextual_closure. apply IHL_contextual_closure.
+  split; apply Lterm_abs with (L := L); apply H1; trivial.
+Qed.
+
+Lemma red_out_Lctx : forall (R : pterm -> pterm -> Prop),
+  L_red_out R -> L_red_out (L_contextual_closure R).
+Proof.
+ intros_all. induction H1.
+ apply L_redex. apply H; trivial.
+ simpl. apply L_app_left; trivial.
+ apply subst_Lterm; trivial.
+ simpl. apply L_app_right; trivial.
+ apply subst_Lterm; trivial.
+ simpl. apply L_abs_in with (L := L \u {{x}}). 
+ intros x0 Fr. apply notin_union in Fr. destruct Fr. 
+ apply notin_singleton in H4.
+ assert (Q: term u). apply Lterm_is_term; trivial.
+ rewrite subst_open_var; trivial.
+ rewrite subst_open_var; trivial.
+ apply H2; trivial.
+Qed.
+
+
+Lemma Lbody_distribute_over_application : forall t u, Lbody (pterm_app t u) <-> Lbody t /\ Lbody u.
+Proof.
+  split.
+    (* -> *)
+    unfold body; unfold open; simpl ; intros; elim H; intros. 
+    split ; exists x; intros; specialize (H0 x0); specialize (H0 H1) ;
+    inversion H0 ; assumption.
+    (* <- *)
+    intros. unfold body in H. unfold body. destruct H.
+    destruct H. destruct H0.
+    exists (x \u x0). intros.
+    unfold open.  simpl. constructor.
+      specialize (H x1) . auto. 
+      specialize (H0 x1) . auto.
+Qed.
+
+
+(** Reduction on lists **)
+
+Lemma Lterm_mult_app : forall t lu, Lterm (t // lu) <-> Lterm t /\ (Lterm %% lu).
+Proof.
+ intros t lu. induction lu; simpl; split; 
+ intro H;  try apply H; try split; trivial.
+ inversion H. apply IHlu; trivial.
+ inversion H. split; trivial. apply IHlu; trivial.
+ destruct H. destruct H0. apply Lterm_app; trivial.
+ apply IHlu; split; trivial.
+Qed.
+
+(* ********************************************************************** *)
+(** Local closure for Lambda terms, recursively defined *)
+
+Fixpoint Llc_at (k:nat) (t:pterm) {struct t} : Prop :=
+  match t with 
+  | pterm_bvar i    => i < k
+  | pterm_fvar x    => True
+  | pterm_app t1 t2 => Llc_at k t1 /\ Llc_at k t2
+  | pterm_abs t1    => Llc_at (S k) t1
+  | pterm_sub t1 t2 => False
+  | pterm_lsub t1 t2 => False
+  end.
+
+Definition Lterm' t := Llc_at 0 t.
+
+Definition Lbody' t := Llc_at 1 t.
+
+(* ********************************************************************** *)
+(** Equivalence of [Lterm and [Lterm'] *)
+
+Lemma Llc_rec_open_var_rec : forall x t k,
+  Llc_at k (open_rec k x t) -> Llc_at (S k) t.
+Proof.
+  induction t; simpl; introv H; auto*.
+  case_nat; simpls~.
+Qed.
+
+Lemma Lterm_to_Lterm' : forall t,
+  Lterm t -> Lterm' t.
+Proof.
+  introv T. induction T; unfold Lterm'; simple~.
+  pick_fresh x. apply~ (@Llc_rec_open_var_rec (pterm_fvar x)). apply~ H0.
+Qed.
+
+Lemma Llc_at_open_var_rec : forall x t k,
+  Llc_at (S k) t -> Llc_at k (open_rec k (pterm_fvar x) t).
+Proof.
+  induction t; simpl; introv H; auto*.
+  case_nat; simpls~.
+  unfold lt in *|-.
+  apply le_lt_or_eq in H.
+  case H.
+  intro H1. apply lt_S_n in H1; trivial.
+  intro H1. assert (n = k).
+  auto. assert (k = n). auto.
+  contradiction.
+Qed. 
+
+Lemma Lterm'_to_Lterm : forall t,
+  Lterm' t -> Lterm t.
+Proof.
+  introv. unfold Lterm'.
+  apply pterm_size_induction with (t := t).
+  (* bvar *)
+  simpl. intros. 
+  assert (~ n < 0). auto with arith.
+  contradiction.
+  (* fvar *)
+  simpl. intros.
+  apply Lterm_var. 
+  (* abs *)
+  simpl. intros.
+  apply Lterm_abs with (L := fv t1).
+  intros x Fr.
+  apply (H t1); trivial.
+  unfold open. 
+  apply Llc_at_open_var_rec; trivial.
+  (* app *)
+  intros t1 t2 IHt1 IHt2 H.
+  simpl in H. apply Lterm_app.
+  apply IHt1; apply H.
+  apply IHt2; apply H.
+  (* sub *)
+  intros. simpl in H1. contradiction.
+  (* sub' *)
+  intros. simpl in H1. contradiction.
+Qed.
+
+
+Lemma Lterm_eq_Lterm' : forall t, Lterm t <-> Lterm' t.
+Proof. intros. split. apply Lterm_to_Lterm'. apply Lterm'_to_Lterm. Qed.
+
+
+(* ********************************************************************** *)
+(** Equivalence of [Lbody] and [Lbody'] *)
+
+Lemma Lbody_to_Lbody' : forall t,
+  Lbody t -> Lbody' t.
+Proof.
+  introv [L H]. pick_fresh x. 
+  applys (@Llc_rec_open_var_rec (pterm_fvar x)).
+  apply Lterm_to_Lterm'. apply~ H.
+Qed.
+
+Lemma Lbody'_to_Lbody : forall t,
+  Lbody' t -> Lbody t.
+Proof.
+  introv B. exists ({}:vars). introv F.
+  apply Lterm'_to_Lterm. apply~ Llc_at_open_var_rec.
+Qed.
+
+Lemma Lbody_eq_Lbody' : forall t, Lbody t <-> Lbody' t.
+Proof. intros. split. apply Lbody_to_Lbody'. apply Lbody'_to_Lbody. Qed.
+
+(* ********************************************************************** *)
+(** Weakening property of [Llc_at] *)
+
+Lemma Llc_at_weaken_ind : forall k1 k2 t,
+  Llc_at k1 t -> k1 <= k2 -> Llc_at k2 t.
+Proof. introv. gen k1 k2. induction t; simpl; introv T Lt; auto*.
+       omega. apply (IHt (S k1) (S k2)); trivial; try omega.
+Qed. 
+
+Lemma Llc_at_weaken : forall k t,
+  Lterm' t -> Llc_at k t.
+Proof. introv H. apply~ (@Llc_at_weaken_ind 0). omega. Qed.
+
+
+Lemma trs_Lctx_app_left : forall R t t' u, Lterm u ->
+                       trans_closure (L_contextual_closure R) t t' ->
+                       trans_closure (L_contextual_closure R) (pterm_app t u) (pterm_app t' u).
+Proof.
+ intros. induction H0. apply one_step_reduction.
+ apply L_app_left; trivial.
+ apply transitive_reduction with (u := pterm_app u0 u); trivial.
+ apply L_app_left; trivial. 
+Qed.
+
+Lemma str_Lctx_app_left : forall R t t' u, Lterm u ->
+                       star_closure (L_contextual_closure R) t t' ->
+                       star_closure (L_contextual_closure R) (pterm_app t u) (pterm_app t' u).
+Proof.
+ intros. induction H0. apply reflexive_reduction. apply star_trans_reduction.
+ apply trs_Lctx_app_left; trivial.
+Qed.
+
+Lemma trs_Lctx_app_right : forall R t u u', Lterm t ->
+                       trans_closure (L_contextual_closure R) u u' ->
+                       trans_closure (L_contextual_closure R) (pterm_app t u) (pterm_app t u').
+Proof.
+ intros. induction H0. apply one_step_reduction.
+ apply L_app_right; trivial.
+ apply transitive_reduction with (u := pterm_app t u); trivial.
+ apply L_app_right; trivial. 
+Qed.
+
+Lemma str_Lctx_app_right : forall R t u u', Lterm t ->
+                       star_closure (L_contextual_closure R) u u' ->
+                       star_closure (L_contextual_closure R) (pterm_app t u) (pterm_app t u').
+Proof.
+ intros. induction H0. apply reflexive_reduction. apply star_trans_reduction.
+ apply trs_Lctx_app_right; trivial.
+Qed.
+
+Lemma Lctx_abs_in_close : forall x R L t t', L_red_regular R -> L_red_out R ->
+                         L_contextual_closure R t t' -> x \notin L ->
+                         L_contextual_closure R (pterm_abs (close t x)) (pterm_abs (close t' x)).
+Proof.
+ intros x R L t t' H0 H1 H2 Fr.
+ apply L_abs_in with (L := L). intros z Fr'. 
+ apply red_out_Lctx in H1. apply L_red_out_to_rename in H1.
+ apply H1 with (x := x). apply fv_close'. apply fv_close'.
+ replace (close t x ^ x) with t. replace (close t' x ^ x) with t'; trivial.
+ apply open_close_var. apply red_regular_Lctx in H0. apply H0 in H2. apply Lterm_is_term. apply H2.
+ apply open_close_var. apply red_regular_Lctx in H0. apply H0 in H2. apply Lterm_is_term. apply H2.
+Qed.
+
+Lemma trs_Lctx_abs_in : forall R L t t', L_red_regular R -> L_red_out R -> 
+                       (forall x, x \notin L ->  trans_closure (L_contextual_closure R) (t ^ x) (t' ^ x)) -> trans_closure (L_contextual_closure R) (pterm_abs t) (pterm_abs t').
+Proof.
+ intros R L t t' H0 H1 H2.  case var_fresh with (L := L \u (fv t) \u (fv t')). intros x Fr.
+ apply notin_union in Fr. destruct Fr. apply notin_union in H. destruct H.
+ assert (Q: trans_closure (L_contextual_closure R) (t ^ x) (t' ^ x)). apply H2; trivial. clear H2.
+ gen_eq t0 : (t ^ x). gen_eq t1 : (t' ^ x). intros Ht0 Ht1.
+ replace t with (close t0 x). replace t' with (close t1 x). clear Ht0 Ht1. induction Q.
+ apply one_step_reduction. apply Lctx_abs_in_close with (L := L); trivial.
+ apply transitive_reduction with (u := pterm_abs (close u x)); trivial.
+ apply Lctx_abs_in_close with (L := L); trivial.
+ rewrite Ht0. rewrite <- close_open_term; trivial. 
+ rewrite Ht1. rewrite <- close_open_term; trivial.
+Qed.
+
+Lemma str_Lctx_abs_in : forall R L t t', L_red_regular R -> L_red_out R -> 
+                       (forall x, x \notin L ->  star_closure (L_contextual_closure R) (t ^ x) (t' ^ x)) -> star_closure (L_contextual_closure R) (pterm_abs t) (pterm_abs t').
+Proof.
+ intros R L t t' H0 H1 H2.  case var_fresh with (L := L \u (fv t) \u (fv t')). intros x Fr.
+ apply notin_union in Fr. destruct Fr. apply notin_union in H. destruct H.
+ assert (Q: star_closure (L_contextual_closure R) (t ^ x) (t' ^ x)). apply H2; trivial. clear H2.
+ gen_eq t0 : (t ^ x). gen_eq t1 : (t' ^ x). intros Ht0 Ht1.
+ replace t with (close t0 x). replace t' with (close t1 x). clear Ht0 Ht1. induction Q.
+ apply reflexive_reduction. apply star_trans_reduction. induction H2.
+ apply one_step_reduction. apply Lctx_abs_in_close with (L := L); trivial.
+ apply transitive_reduction with (u := pterm_abs (close u x)); trivial.
+ apply Lctx_abs_in_close with (L := L); trivial.
+ rewrite Ht0. rewrite <- close_open_term; trivial. 
+ rewrite Ht1. rewrite <- close_open_term; trivial.
+Qed.
+
+
 (******)
+
+
 
 Lemma left_trans_app_Beta: forall t u v,  Lterm t  ->   
       u -->Beta+ v -> pterm_app u t -->Beta+ pterm_app v t.
@@ -99,6 +432,294 @@ Proof.
  intros; apply str_Lctx_abs_in with (L := L); trivial.
  apply L_beta_regular.
  apply L_beta_red_out.
+Qed.
+
+(** Induction Principles *)
+
+Lemma Lbody_size_induction :
+ forall P : pterm -> Prop,
+ (P (pterm_bvar 0)) ->
+ (forall x, P (pterm_fvar x)) ->
+ (forall t1, (Llc_at 2 t1) ->
+    (forall t2 x, x \notin fv t2 -> pterm_size t2 = pterm_size t1 ->
+    Lbody (open_rec 1 (pterm_fvar x) t2) -> P (open_rec 1 (pterm_fvar x) t2)) -> P (pterm_abs t1)) ->
+ (forall t1 t2, Lbody t1 -> Lbody t2 -> P t1 -> P t2 -> P (pterm_app t1 t2)) ->
+ (forall t, Lbody t -> P t).
+Proof.
+  intros P Ha Hb Hc Hd t.
+  gen_eq n: (pterm_size t). gen t.
+  induction n using peano_induction.
+  introv Eq B. subst. destruct t. 
+     (* bvar *)
+     generalize B; clear B; case n.
+     intro B; apply Ha.
+     intros n' H'; apply not_Lbody_Sn in H'; contradiction.
+     (* fvar *)
+     apply Hb.
+     (* app *)
+     apply~ Hd; 
+     apply Lbody_distribute_over_application in B.
+     apply B. apply B.
+     apply~ H. simpl; omega. 
+     apply B. apply~ H. simpl; omega.
+     apply B.
+     (* abs *)
+     apply* Hc.
+     apply Lbody_to_Lbody' in B.
+     unfold Lbody' in B. simpl in B; trivial.
+     introv Fr Eq.
+     apply~ H. rewrite <- pterm_size_open_var. simpl. omega.
+     (* sub *)
+     apply Lbody_to_Lbody' in B. unfold Lbody' in B. simpl in B.
+     contradiction.
+     (* sub' *)
+     apply Lbody_to_Lbody' in B. unfold Lbody' in B. simpl in B.
+     contradiction.
+Qed.
+
+Lemma Lterm_size_induction :
+ forall P : pterm -> Prop,
+ (forall x, P (pterm_fvar x)) ->
+ (forall t1 t2,
+    Lterm t1 -> P t1 -> Lterm t2 -> P t2 -> P (pterm_app t1 t2)) ->
+ (forall t1,
+    Lbody t1 ->
+    (forall t2 x, x \notin fv t2 -> pterm_size t2 = pterm_size t1 ->
+      Lterm (t2 ^ x) -> P (t2 ^ x)) ->
+    P (pterm_abs t1)) ->
+ (forall t, Lterm t -> P t).
+Proof.
+  intros P Ha Hb Hc t.
+  gen_eq n: (pterm_size t). gen t.
+  induction n using peano_induction.
+  introv Eq T. subst. inverts T. 
+     apply Ha.
+     (* app *)
+     apply~ Hb. apply~ H. simpl; omega. apply~ H. simpl; omega.
+     (* abs *)
+     apply* Hc.
+       introv. exists L. trivial.
+       introv Fr Eq T.
+       apply~ H. unfold open.
+      rewrite <- pterm_size_open_var. simpl. omega.
+ Qed.
+
+Lemma Lterm_size_induction2 :
+ forall P : pterm -> Prop,
+ (forall x l, (forall u, In u l -> (Lterm u /\ P u)) -> P ((pterm_fvar x) // l)) ->
+ (forall t1 l, (forall u, In u l -> (Lterm u /\ P u)) -> Lbody t1 ->
+  (forall t2 x, x \notin fv t2 -> pterm_size t2 = pterm_size t1 -> Lterm (t2 ^ x) -> P (t2 ^ x)) ->
+      P ((pterm_abs t1) // l)) ->
+ (forall l t, (forall u, In u l -> (Lterm u /\ P u)) -> Lterm t -> P (t // l)).
+Proof.
+ intros. generalize H2.  intro T. generalize l H1 H2. clear l H1 H2.
+ apply Lterm_size_induction with (t := t); trivial; intros.
+ apply H; trivial.
+ replace (pterm_app t1 t2 // l) with (t1 // l ++ (t2 :: nil)).  
+ apply H2. intros. apply in_app_iff in H7. destruct H7.
+ apply H5; trivial. simpl in H7. destruct H7; try contradiction.
+ rewrite <- H7. clear H7. inversion H6. split; trivial.
+ assert (Q : P (t2 // nil)). 
+   apply H4; simpl; trivial; intros. contradiction. 
+ simpl in Q. trivial. trivial. 
+ rewrite mult_app_append. trivial.
+ apply H0; trivial. intros.
+ assert (Q : P (t2 ^ x // nil)).
+   apply H2; simpl; trivial; intros. contradiction.
+ simpl in Q. trivial.
+Qed.
+
+
+Lemma Lterm_size_induction3 :
+ forall P : pterm -> Prop,
+ (forall x l, (forall u, In u l -> (Lterm u /\ P u)) -> P ((pterm_fvar x) // l)) ->
+ (forall t1 l, (forall u, In u l -> (Lterm u /\ P u)) -> Lbody t1 ->
+  (forall t2 x, x \notin fv t2 -> pterm_size t2 = pterm_size t1 -> Lterm (t2 ^ x) -> P (t2 ^ x)) ->
+      P ((pterm_abs t1) // l)) ->
+ (forall t, Lterm t -> P t).
+Proof. 
+ intros. replace t with (t // nil).
+ apply Lterm_size_induction2; simpl; trivial.
+ intros; contradiction. 
+ simpl. trivial.
+Qed.
+
+
+Lemma Llc_at_bswap : forall n k t, S k < n -> Llc_at n t -> Llc_at n (bswap_rec k t).
+Proof.
+ intros n k t. 
+ generalize n k; clear n k.
+ induction t.
+ (* bvar *)
+ intros n' k H0 H1. simpl in H1.
+ unfolds bswap_rec. 
+ case (k === n). intro H2.
+ rewrite H2. simpl. omega. intro H2.
+ case (S k === n). intro H3. simpl. omega. intro H3. 
+ simpl. trivial.
+ (* fvar *)
+ intros n k H0 H1. simpl in *|-*. trivial.
+ (* app *)
+ intros n k H0 H1. simpl in *|-*. destruct H1. split.
+ apply IHt1; trivial. apply IHt2; trivial.
+ (* abs *)
+ intros n k H0 H1. simpl in *|-*.
+ apply IHt; try omega; trivial.
+ (* sub *)
+ intros n k H0 H1. simpl in *|-*. contradiction. 
+ (* sub' *)
+ intros n k H0 H1. simpl in *|-*. contradiction. 
+Qed.
+
+Lemma Llc_at_open : forall n t u, Lterm u -> (Llc_at (S n) t <-> Llc_at n (open_rec n u t)).
+Proof.
+ intros n t u T. split.
+(* -> *)
+ generalize n; clear n.
+ induction t.
+ (* bvar *)
+ intros n' H0. unfolds open_rec.
+ case (n' === n). intro H1.
+ rewrite H1 in H0. rewrite H1. simpl in *|-*. 
+ apply Lterm_to_Lterm' in T. unfold Lterm' in T.
+ apply Llc_at_weaken_ind with (k1 := 0); try omega; trivial.
+ intro H1. simpl in *|-*. omega.
+ (* fvar *)
+ intros n H. simpl. trivial.
+ (* app *)
+ intros n H. simpl in *|-*.
+ case H; clear H; intros Ht1 Ht2; split.
+ apply (IHt1 n Ht1). 
+ apply (IHt2 n Ht2).
+ (* abs *)
+ intros n H. simpl in *|-*.
+ apply (IHt (S n) H).
+ (* sub *)
+ intros n H. simpl in *|-*. contradiction.
+ (* sub' *)
+ intros n H. simpl in *|-*. contradiction.
+(* <- *)
+ generalize n; clear n.
+ induction t.
+ (* bvar *)
+ intros n' H0. simpl in H0.
+ case (n' === n) in H0. simpl. omega.
+ simpl in *|-*. omega.
+ (* fvar *)
+ simpl. trivial. 
+ (* app *)
+ simpl in *|-*. intros n H.
+ case H; clear H; intros Ht1 Ht2; split.
+ apply (IHt1 n Ht1). 
+ apply (IHt2 n Ht2).
+ (* abs *)
+ simpl in *|-*. intros n H. 
+ apply (IHt (S n) H).
+ (* sub *)
+ simpl in *|-*. intros n H. contradiction. 
+ (* sub' *)
+ simpl in *|-*. intros n H. contradiction.
+Qed.
+
+Lemma L_SN_app : forall n R t u, L_red_regular R ->  Lterm t -> Lterm u -> 
+               SN_ind n (L_contextual_closure R) (pterm_app t u) ->
+               SN_ind n (L_contextual_closure R) t /\ SN_ind n (L_contextual_closure R) u.
+ Proof.
+ intros n R t u Reg. 
+ generalize t u; clear t u.  
+ induction n.  intros. split; rewrite <- NF_eq_SN0 in *|-*; unfold NF in *|-*. 
+ intros t' H'. apply (H1 (pterm_app t' u)). apply L_app_left; trivial.
+ intros u' H'. apply (H1 (pterm_app t u')). apply L_app_right; trivial.
+ intros t u Tt Tu H. destruct H. split. 
+ apply SN_intro. intros t' H'. exists n. split; try omega. 
+ apply IHn with (t := t') (u := u); trivial. apply red_regular_Lctx in Reg.
+ apply Reg in H'. apply H'. case (H (pterm_app t' u)). apply L_app_left; trivial. 
+ intros k H''. apply WSN with (k := k). omega. apply H''.
+ apply SN_intro. intros u' H'. exists n. split; try omega. 
+ apply IHn with (t := t) (u := u'); trivial. apply red_regular_Lctx in Reg.
+ apply Reg in H'. apply H'. case (H (pterm_app t u')). apply L_app_right; trivial. 
+ intros k H''. apply WSN with (k := k). omega. apply H''.
+Qed. 
+
+
+Lemma L_SN_abs : forall x n R t, L_red_regular R -> L_red_out R -> 
+               SN_ind n (L_contextual_closure R) (pterm_abs t) ->
+               x \notin (fv t) -> SN_ind n (L_contextual_closure R) (t ^ x).
+Proof.
+ intros x n R t Reg Out.
+ generalize t; clear t.
+ apply red_regular_Lctx in Reg. 
+ apply red_out_Lctx in Out. 
+ apply L_red_out_to_rename in Out.
+ induction n. intros. 
+ apply SN0_to_NF in H. 
+ apply NF_to_SN0; unfold NF in *|-*.
+ intros t' H'. gen_eq t0 : (close t' x). intro H1.
+ replace t' with (t0 ^ x) in H'.
+ assert (Q: L_contextual_closure R (pterm_abs t) (pterm_abs t0)).
+    apply L_abs_in with (L := {{x}}). intros z H2. 
+    apply notin_singleton in H2. apply Out with (x := x); trivial.
+    rewrite H1. apply fv_close'.
+ assert (Q': ~ L_contextual_closure R (pterm_abs t) (pterm_abs t0)).
+    apply H.
+ contradiction. rewrite H1. rewrite open_close_var with (x := x).
+ reflexivity. apply Reg in H'. apply Lterm_is_term. apply H'.
+ intros. destruct H. apply SN_intro.
+ intros. exists n. split; try omega.
+ gen_eq t0 : (close t' x). intro H2.
+ replace t' with (t0 ^ x). replace t' with (t0 ^ x) in H1.
+ apply IHn; trivial. case (H (pterm_abs t0)); trivial.
+ apply L_abs_in with (L := {{x}}).
+ intros z H3. apply notin_singleton in H3. 
+ apply Out with (x := x); trivial.
+ rewrite H2. apply fv_close'.
+ intros k H3. apply WSN with (k := k); try omega.
+ apply H3. rewrite H2. apply fv_close'.
+ rewrite H2. rewrite open_close_var with (x := x).
+ reflexivity. apply Lterm_is_term. apply Reg in H1. apply H1.
+ rewrite H2. rewrite open_close_var with (x := x).
+ reflexivity. apply Lterm_is_term. apply Reg in H1. apply H1. 
+Qed.
+
+
+Lemma L_SN_mult_app : forall n R t l, L_red_regular R ->  Lterm t -> Lterm %% l -> 
+               SN_ind n (L_contextual_closure R) (t // l) ->
+               SN_ind n (L_contextual_closure R) t /\ SN_ind n (L_contextual_closure R) %% l.
+Proof.
+ intros n R t l Reg. generalize n t; clear n t.
+ induction l; simpl. intros n t T H0 H. split; trivial.
+ intros n t T H0 H. destruct H0. apply L_SN_app in H; trivial. destruct H.
+ assert (Q : SN_ind n (L_contextual_closure R) t /\ SN_ind n (L_contextual_closure R) %% l). 
+  apply IHl; trivial.
+ clear IHl. destruct Q. split; trivial. split; trivial.
+ rewrite Lterm_mult_app. split; trivial. 
+Qed. 
+
+Lemma Lctx_red_h_mult_app : forall R t t' lu, Lterm %% lu -> (L_contextual_closure R) t t' -> (L_contextual_closure R) (t // lu) (t' // lu).
+Proof.
+ intros R t t' lu Tlu H. induction lu; simpl in *|-*; trivial.
+ destruct Tlu. apply L_app_left; trivial.
+ apply IHlu; trivial.
+Qed. 
+
+Lemma Lctx_red_t_mult_app : forall R t lu lu', Lterm t -> Lterm %% lu -> R_list (L_contextual_closure R) lu lu' -> (L_contextual_closure R) (t // lu) (t // lu').
+Proof.
+ intros R t lu lu' Tt Tlu H. unfold R_list in H.
+ case H; clear H; intros t0 H.
+ case H; clear H; intros t1 H.
+ case H; clear H; intros l0 H.
+ case H; clear H; intros l1 H.
+ destruct H. destruct H0. 
+ rewrite H. rewrite H0. rewrite H in Tlu. 
+ clear H H0. induction l0; simpl. destruct l1; simpl. 
+ apply L_app_right; trivial.
+ apply L_app_right; trivial. 
+ simpl in Tlu. apply Lterm_app. rewrite Lterm_mult_app. 
+ destruct Tlu. destruct H0.
+ split; trivial. apply Tlu.
+ simpl in Tlu. destruct Tlu. 
+ apply L_app_left; trivial.
+ apply IHl0; trivial. 
 Qed.
 
 
