LambdaES_Defs.v
@@ -1,27 +1,27 @@
 (***************************************************************************
-* Formalization of ES calculi						   *		
+* Formalizing SN for lambda_ex						   *		
 *									   *
 * Definitions of explicit substitutions 				   *
 * Brian Aydemir & Arthur Chargueraud, July 2007              	   	   *
 * Fabien Renaud, 2011							   *
-* Flávio L. C. de Moura, 2015                                              *
+* Flávio L. C. de Moura, 2016                                              *
 ***************************************************************************)
 
 Set Implicit Arguments.
 Require Import Metatheory.
 
-(** Grammar of pre-terms. *)
+(** Pre-terms are expressions arbitrarily built from the following constructors: *)
 Inductive pterm : Set :=
   | pterm_bvar : nat -> pterm
   | pterm_fvar : var -> pterm
   | pterm_app  : pterm -> pterm -> pterm
   | pterm_abs  : pterm -> pterm
   | pterm_sub : pterm -> pterm -> pterm 
-  | pterm_sub' : pterm -> pterm -> pterm  (* labeled explicit substitutions *)
-.
+  | pterm_lsub : pterm -> pterm -> pterm.
+(** Bound and free variables have different constructors. In fact, [pterm_bvar] will be used to represent bound variables that are codified by deBruijn indexes. Free variables are represented with names, so the free variable x will be denoted by [pterm_fvar x]. The constructor [pterm_app] and [pterm_abs] are used respectively for representing applications and abstractions. Explicit substitutions appear in two flavors: with or without marks. Therefore, [pterm_sub t u] represents the term [t] with an explicit substitution [u], while [pterm_lsub t u] is the constructor for labeled substitutions. The adopted notations for explicit substitutions are as follows: *)
 
 Notation "t [ u ]" := (pterm_sub t u) (at level 70).
-Notation "t [[ u ]]" := (pterm_sub' t u) (at level 70).
+Notation "t [[ u ]]" := (pterm_lsub t u) (at level 70).
 
 (** Opening up abstractions and substitutions *)
 Fixpoint open_rec (k : nat) (u : pterm) (t : pterm) {struct t} : pterm :=
@@ -31,14 +31,14 @@ Fixpoint open_rec (k : nat) (u : pterm) (t : pterm) {struct t} : pterm :=
   | pterm_app t1 t2 => pterm_app (open_rec k u t1) (open_rec k u t2)
   | pterm_abs t1    => pterm_abs (open_rec (S k) u t1)
   | pterm_sub t1 t2 => pterm_sub (open_rec (S k) u t1) (open_rec k u t2)
-  | pterm_sub' t1 t2 => pterm_sub' (open_rec (S k) u t1) (open_rec k u t2)
+  | pterm_lsub t1 t2 => pterm_lsub (open_rec (S k) u t1) (open_rec k u t2)
   end.
 
 Definition open t u := open_rec 0 u t.
 
 Notation "{ k ~> u } t" := (open_rec k u t) (at level 67).
-Notation "t ^^ u" := (open t u) (at level 67). (* verificar *)
-Notation "t ^ x" := (open t (pterm_fvar x)).   (* verificar *)
+Notation "t ^^ u" := (open t u) (at level 67). 
+Notation "t ^ x" := (open t (pterm_fvar x)).   
 
 (** Variable closing *)
 Fixpoint close_rec  (k : nat) (x : var) (t : pterm) {struct t} : pterm :=
@@ -48,7 +48,7 @@ Fixpoint close_rec  (k : nat) (x : var) (t : pterm) {struct t} : pterm :=
   | pterm_app t1 t2 => pterm_app (close_rec k x t1) (close_rec k x t2)
   | pterm_abs t1    => pterm_abs (close_rec (S k) x t1)
   | pterm_sub t1 t2 => pterm_sub (close_rec (S k) x t1) (close_rec k x t2)
-  | pterm_sub' t1 t2 => pterm_sub' (close_rec (S k) x t1) (close_rec k x t2)
+  | pterm_lsub t1 t2 => pterm_lsub (close_rec (S k) x t1) (close_rec k x t2)
   end.
 
 Definition close t x := close_rec 0 x t.
@@ -60,7 +60,7 @@ Fixpoint fv (t : pterm) {struct t} : vars :=
   | pterm_app t1 t2 => (fv t1) \u (fv t2)
   | pterm_abs t1    => (fv t1)
   | pterm_sub t1 t2 => (fv t1) \u (fv t2)
-  | pterm_sub' t1 t2 => (fv t1) \u (fv t2)
+  | pterm_lsub t1 t2 => (fv t1) \u (fv t2)
   end.
 
   
@@ -72,7 +72,7 @@ Fixpoint bswap_rec (k : nat) (t : pterm) {struct t} : pterm :=
   | pterm_app t1 t2 => pterm_app (bswap_rec k t1) (bswap_rec k t2)
   | pterm_abs t1    => pterm_abs (bswap_rec (S k) t1)
   | pterm_sub t1 t2 => pterm_sub (bswap_rec (S k) t1) (bswap_rec k t2)
-  | pterm_sub' t1 t2 => pterm_sub' (bswap_rec (S k) t1) (bswap_rec k t2)
+  | pterm_lsub t1 t2 => pterm_lsub (bswap_rec (S k) t1) (bswap_rec k t2)
   end.
 
 Definition bswap t := bswap_rec 0 t.
@@ -86,7 +86,7 @@ Fixpoint swap (x y : var) (t : pterm) {struct t} : pterm :=
   | pterm_app t1 t2 => pterm_app (swap x y t1) (swap x y t2)
   | pterm_abs t1    => pterm_abs (swap x y t1)
   | pterm_sub t1 t2 => pterm_sub (swap x y t1) (swap x y t2)
-  | pterm_sub' t1 t2 => pterm_sub' (swap x y t1) (swap x y t2)
+  | pterm_lsub t1 t2 => pterm_lsub (swap x y t1) (swap x y t2)
   end.
 
 Notation "[( x , y )] t" := (swap x y t) (at level 67).
@@ -102,7 +102,7 @@ Fixpoint pterm_size (t : pterm) {struct t} : nat :=
  | pterm_abs t1    => 1 + (pterm_size t1)
  | pterm_app t1 t2 => 1 + (pterm_size t1) + (pterm_size t2)
  | pterm_sub t1 t2 => 1 + (pterm_size t1) + (pterm_size t2)
- | pterm_sub' t1 t2 => 1 + (pterm_size t1) + (pterm_size t2)
+ | pterm_lsub t1 t2 => 1 + (pterm_size t1) + (pterm_size t2)
  end.
 
 Lemma pterm_size_non_null : forall t, pterm_size t > 0.
@@ -117,14 +117,71 @@ Proof.
 Qed.
 
 (** Implicit substitution, for free names *)
-Fixpoint subst (z : var) (u : pterm) (t : pterm) : pterm :=
+Fixpoint m_sb (z : var) (u : pterm) (t : pterm) : pterm :=
   match t with
   | pterm_bvar i    => pterm_bvar i
   | pterm_fvar x    => if x == z then u else (pterm_fvar x)
-  | pterm_abs t1    => pterm_abs (subst z u t1)
-  | pterm_app t1 t2 => pterm_app (subst z u t1) (subst z u t2)
-  | pterm_sub t1 t2 => pterm_sub (subst z u t1) (subst z u t2)
-  | pterm_sub' t1 t2 => pterm_sub' (subst z u t1) (subst z u t2)
+  | pterm_abs t1    => pterm_abs (m_sb z u t1)
+  | pterm_app t1 t2 => pterm_app (m_sb z u t1) (m_sb z u t2)
+  | pterm_sub t1 t2 => pterm_sub (m_sb z u t1) (m_sb z u t2)
+  | pterm_lsub t1 t2 => pterm_lsub (m_sb z u t1) (m_sb z u t2)
   end.
-Notation "[ z ~> u ] t" := (subst z u t) (at level 62).
+Notation "[ z ~> u ] t" := (m_sb z u t) (at level 62).
+
+(** ES terms are expressions without dangling deBruijn indexes. *)
+Inductive term : pterm -> Prop :=
+  | term_var : forall x,
+      term (pterm_fvar x)
+  | term_app : forall t1 t2,
+      term t1 -> 
+      term t2 -> 
+      term (pterm_app t1 t2)
+  | term_abs : forall L t1,
+      (forall x, x \notin L -> term (t1 ^ x)) ->
+      term (pterm_abs t1)
+  | term_sub : forall L t1 t2,
+     (forall x, x \notin L -> term (t1 ^ x)) ->
+      term t2 -> 
+      term (pterm_sub t1 t2).
+
+Lemma term_size_non_null : forall t, term t -> pterm_size t > 0.
+Proof.
+  intros t Ht. destruct t. inversion Ht.
+  simpl; auto.  
+  simpl; auto.  
+  simpl. omega.
+  simpl. omega.
+  simpl. omega. inversion Ht.
+Qed.  
+
+(** Body *) 
+Definition body t := exists L, forall x, x \notin L -> term (t ^ x).
+
+Hint Constructors term.
+
+(** Pure lambda terms. *)
+Inductive Lterm : pterm -> Prop :=
+  | Lterm_var : forall x,
+      Lterm (pterm_fvar x)
+  | Lterm_app : forall t1 t2,
+      Lterm t1 -> 
+      Lterm t2 -> 
+      Lterm (pterm_app t1 t2)
+  | Lterm_abs : forall L t1,
+      (forall x, x \notin L -> Lterm (t1 ^ x)) ->
+      Lterm (pterm_abs t1).
+
+Lemma Lterm_size_non_null : forall t, Lterm t -> pterm_size t > 0.
+Proof.
+  intros t Ht. destruct t.
+  inversion Ht.
+  simpl; auto.  
+  simpl. omega.
+  simpl. omega. inversion Ht. inversion Ht.
+Qed.  
+
+(** Body for pure lambda terms *) 
+Definition Lbody t := exists L, forall x, x \notin L -> Lterm (t ^ x).
+
+Hint Constructors Lterm.
 
