LambdaES_Infra.v
@@ -5,12 +5,13 @@
 *									   *
 * Arthur Chargu\u00e9raud, 2007						   *
 * Fabien Renaud & St\u00e9phane Zimmerman, 2011				   *
-* Flávio L. C. de Moura, 2015                                              *
+* Flávio L. C. de Moura, 2016                                              *
 ***************************************************************************)
 
 
 Set Implicit Arguments.
-Require Import  Metatheory LambdaES_Defs LambdaES_Tac LambdaES_FV.
+Require Import  Metatheory LambdaES_Defs. 
+Require Import Rewriting LambdaES_Tac LambdaES_FV.
 Require Import Arith List. 
 
 (* ********************************************************************** *)
@@ -45,54 +46,6 @@ Tactic Notation "apply_fresh" constr(T) :=
   apply_fresh_base T gather_vars ltac_no_arg.
 Tactic Notation "apply_fresh" "*" constr(T) :=
   apply_fresh T; auto_star.
-
-(** ES terms are expressions without dangling deBruijn indexes. *)
-Inductive term : pterm -> Prop :=
-  | term_var : forall x,
-      term (pterm_fvar x)
-  | term_app : forall t1 t2,
-      term t1 -> 
-      term t2 -> 
-      term (pterm_app t1 t2)
-  | term_abs : forall L t1,
-      (forall x, x \notin L -> term (t1 ^ x)) ->
-      term (pterm_abs t1)
-  | term_sub : forall L t1 t2,
-     (forall x, x \notin L -> term (t1 ^ x)) ->
-      term t2 -> 
-      term (pterm_sub t1 t2).
-
-Lemma term_size_non_null : forall t, term t -> pterm_size t > 0.
-Proof.
-  intros t Ht. destruct t.
-  simpl; auto.  
-  simpl; auto.  
-  simpl. omega.
-  simpl. omega.
-  simpl. omega.
-  simpl. omega.
-Qed.  
-
-(** Pure lambda terms. *)
-Inductive Lterm : pterm -> Prop :=
-  | Lterm_var : forall x,
-      Lterm (pterm_fvar x)
-  | Lterm_app : forall t1 t2,
-      Lterm t1 -> 
-      Lterm t2 -> 
-      Lterm (pterm_app t1 t2)
-  | Lterm_abs : forall L t1,
-      (forall x, x \notin L -> Lterm (t1 ^ x)) ->
-      Lterm (pterm_abs t1).
-
-(** Body *) 
-Definition body t := exists L, forall x, x \notin L -> term (t ^ x).
-
-(** Body for pure lambda terms *) 
-Definition Lbody t := exists L, forall x, x \notin L -> Lterm (t ^ x).
-
-Hint Constructors term.
-Hint Constructors Lterm.
 
 (******************************************************)
 (** Lemmas. *)
@@ -245,22 +198,6 @@ Proof.
       specialize (H x1) . auto. 
       specialize (H0 x1) . auto.
 Qed.
-
-Lemma Lbody_distribute_over_application : forall t u, Lbody (pterm_app t u) <-> Lbody t /\ Lbody u.
-Proof.
-  split.
-    (* -> *)
-    unfold body; unfold open; simpl ; intros; elim H; intros. 
-    split ; exists x; intros; specialize (H0 x0); specialize (H0 H1) ;
-    inversion H0 ; assumption.
-    (* <- *)
-    intros. unfold body in H. unfold body. destruct H.
-    destruct H. destruct H0.
-    exists (x \u x0). intros.
-    unfold open.  simpl. constructor.
-      specialize (H x1) . auto. 
-      specialize (H0 x1) . auto.
-Qed.
   
 Lemma term_abs_term : forall t, term t -> term (pterm_abs t).
 Proof.
@@ -337,101 +274,27 @@ Proof.
   rewrite <- open_close_var with (x:=x) ; auto.
   apply notin_fv_close.
 Qed.
-
+  
 (** Auxiliary lemmas. *)
 
 Lemma term_distribute_over_application : forall t u, term (pterm_app t u) <-> term t /\ term u.
 Proof.
   split.
-    (* -> *)
-  intro. split; 
-  inversion H; assumption.
-  (* <- *)
-  intro.
-  destruct H.
+  intro. split; inversion H; assumption.
+  intro. destruct H.
   apply term_app; assumption.
 Qed.
 
-Lemma Lterm_is_term: forall t, Lterm t -> term t.
-Proof.
- intros. induction H; trivial.
- apply term_distribute_over_application; split; trivial.
- apply body_to_term_abs; trivial. unfold body.
- exists L; trivial.
-Qed.
-
-Lemma Lbody_is_body: forall t, Lbody t -> body t.
-Proof.
- intros. unfold body. unfold Lbody in H.
- case H; clear H; intros L H. exists L.
- intros x H'. apply Lterm_is_term.
- apply H; trivial.
-Qed.
-
-Lemma subst_Lterm : forall t z u,
-  Lterm u -> Lterm t -> Lterm ([z ~> u]t).
-Proof.
-  induction 2; simpls*.
-  case_var*. apply_fresh Lterm_abs. rewrite* subst_open_var. apply Lterm_is_term; trivial.
-Qed.
-Hint Resolve subst_Lterm.
-
-Lemma Lbody_open_term : forall t u, Lbody t -> Lterm u -> Lterm (t ^^ u).
-Proof.
- intros. destruct H. case var_fresh with (L := x \u (fv t)).
- intros y Fr. rewrite* (@subst_intro y).
-Qed.
 Hint Resolve body_open_term.
 
 Lemma not_body_Sn: forall n, ~(body (pterm_bvar (S n))).
 Proof.
-  intro n.
-  intro H. 
-  elim H.
-  intro L.
-  intro H1.
-  pick_fresh z.
+  intro n. intro H. elim H.
+  intro L. intro H1. pick_fresh z.
   assert (z \notin L). auto.
   assert (term (pterm_bvar (S n) ^ z)).
-  apply H1.
-  assumption.
-  inversion H2.
-Qed.
-
-Lemma not_Lbody_Sn: forall n, ~(Lbody (pterm_bvar (S n))).
-Proof.
-  intro n.
-  intro H. 
-  elim H.
-  intro L.
-  intro H1.
-  pick_fresh z.
-  assert (z \notin L). auto.
-  assert (Lterm (pterm_bvar (S n) ^ z)).
-  apply H1.
-  assumption.
-  inversion H2.
-Qed.
-
-Lemma body_to_term: forall t x, x \notin fv t -> body t -> term (t^x).
-Proof.
-  intros.
-  inversion* H0.
-Qed.
-
-(*
-Lemma term_to_body: forall t x, x \notin fv t -> term (t^x) -> body t.
-Proof.
-  induction t.
-  intros.
-  unfold body.  
-  simpl in H.
-  exists {}.
-  intros.
-  inversion H0.
-  inversion H3.
-  unfold open.
- *) 
+  apply H1. assumption. inversion H2.
+Qed.  
   
 (* ********************************************************************** *)
 (** Induction Principles Part 1*)
@@ -528,35 +391,6 @@ Proof.
   apply Hsub'.
 Qed.
 
-Lemma pterm_induction' :
- forall P : pterm -> Prop,
- (forall n, P (pterm_bvar n)) ->
- (forall x, P (pterm_fvar x)) ->
- (forall t1,
-    (forall x, x \notin (fv t1) -> P (t1 ^ x)) -> P (pterm_abs t1)) ->
- (forall t1 t2, P t1 -> P t2 -> P (pterm_app t1 t2)) ->
- (forall t1 t2, P t2 -> 
-    (forall x, x \notin fv t1 -> P (t1 ^ x)) -> P (t1[t2])) ->
-  (forall t1 t2, P t2 -> 
-    (forall x, x \notin fv t1 -> P (t1 ^ x)) -> P (t1[[t2]])) -> 
- (forall t, P t).
-Proof.
-  intros P Hbvar Hfvar Habs Happ Hes Hles.
-  induction t using pterm_size_induction.
-  apply Hbvar.
-  apply Hfvar.
-  apply Habs.
-  intros x H1.
-  apply H. assumption. reflexivity.
-  apply Happ; assumption. 
-  apply Hes. assumption.
-  intros x H1.
-  apply H. assumption. reflexivity.
-  apply Hles. assumption.
-  intros x H1.
-  apply H. assumption. reflexivity.
-Qed.
-  
 Fixpoint lc_at (k:nat) (t:pterm) {struct t} : Prop :=
   match t with 
   | pterm_bvar i    => i < k
@@ -564,30 +398,14 @@ Fixpoint lc_at (k:nat) (t:pterm) {struct t} : Prop :=
   | pterm_app t1 t2 => lc_at k t1 /\ lc_at k t2
   | pterm_abs t1    => lc_at (S k) t1
   | pterm_sub t1 t2 => (lc_at (S k) t1) /\ lc_at k t2
-  | pterm_sub' t1 t2 => False
+  | pterm_lsub t1 t2 => False
   end.
 
 Definition term' t := lc_at 0 t.
 
 Definition body' t := lc_at 1 t.
 
-(* ********************************************************************** *)
-(** Local closure for Lambda terms, recursively defined *)
 
-Fixpoint Llc_at (k:nat) (t:pterm) {struct t} : Prop :=
-  match t with 
-  | pterm_bvar i    => i < k
-  | pterm_fvar x    => True
-  | pterm_app t1 t2 => Llc_at k t1 /\ Llc_at k t2
-  | pterm_abs t1    => Llc_at (S k) t1
-  | pterm_sub t1 t2 => False
-  | pterm_sub' t1 t2 => False
-  end.
-
-Definition Lterm' t := Llc_at 0 t.
-
-Definition Lbody' t := Llc_at 1 t.
-  
 (* ********************************************************************** *)
 (** Equivalence of [term and [term'] *)
 
@@ -685,92 +503,6 @@ Lemma body_eq_body' : forall t, body t <-> body' t.
 Proof. intros. split. apply body_to_body'. apply body'_to_body. Qed.
 
 
-(* ********************************************************************** *)
-(** Equivalence of [Lterm and [Lterm'] *)
-
-Lemma Llc_rec_open_var_rec : forall x t k,
-  Llc_at k (open_rec k x t) -> Llc_at (S k) t.
-Proof.
-  induction t; simpl; introv H; auto*.
-  case_nat; simpls~.
-Qed.
-
-Lemma Lterm_to_Lterm' : forall t,
-  Lterm t -> Lterm' t.
-Proof.
-  introv T. induction T; unfold Lterm'; simple~.
-  pick_fresh x. apply~ (@Llc_rec_open_var_rec (pterm_fvar x)). apply~ H0.
-Qed.
-
-Lemma Llc_at_open_var_rec : forall x t k,
-  Llc_at (S k) t -> Llc_at k (open_rec k (pterm_fvar x) t).
-Proof.
-  induction t; simpl; introv H; auto*.
-  case_nat; simpls~.
-  unfold lt in *|-.
-  apply le_lt_or_eq in H.
-  case H.
-  intro H1. apply lt_S_n in H1; trivial.
-  intro H1. assert (n = k).
-  auto. assert (k = n). auto.
-  contradiction.
-Qed. 
-
-Lemma Lterm'_to_Lterm : forall t,
-  Lterm' t -> Lterm t.
-Proof.
-  introv. unfold Lterm'.
-  apply pterm_size_induction with (t := t).
-  (* bvar *)
-  simpl. intros. 
-  assert (~ n < 0). auto with arith.
-  contradiction.
-  (* fvar *)
-  simpl. intros.
-  apply Lterm_var. 
-  (* abs *)
-  simpl. intros.
-  apply Lterm_abs with (L := fv t1).
-  intros x Fr.
-  apply (H t1); trivial.
-  unfold open. 
-  apply Llc_at_open_var_rec; trivial.
-  (* app *)
-  intros t1 t2 IHt1 IHt2 H.
-  simpl in H. apply Lterm_app.
-  apply IHt1; apply H.
-  apply IHt2; apply H.
-  (* sub *)
-  intros. simpl in H1. contradiction.
-  (* sub' *)
-  intros. simpl in H1. contradiction.
-Qed.
-
-
-Lemma Lterm_eq_Lterm' : forall t, Lterm t <-> Lterm' t.
-Proof. intros. split. apply Lterm_to_Lterm'. apply Lterm'_to_Lterm. Qed.
-
-
-(* ********************************************************************** *)
-(** Equivalence of [Lbody] and [Lbody'] *)
-
-Lemma Lbody_to_Lbody' : forall t,
-  Lbody t -> Lbody' t.
-Proof.
-  introv [L H]. pick_fresh x. 
-  applys (@Llc_rec_open_var_rec (pterm_fvar x)).
-  apply Lterm_to_Lterm'. apply~ H.
-Qed.
-
-Lemma Lbody'_to_Lbody : forall t,
-  Lbody' t -> Lbody t.
-Proof.
-  introv B. exists ({}:vars). introv F.
-  apply Lterm'_to_Lterm. apply~ Llc_at_open_var_rec.
-Qed.
-
-Lemma Lbody_eq_Lbody' : forall t, Lbody t <-> Lbody' t.
-Proof. intros. split. apply Lbody_to_Lbody'. apply Lbody'_to_Lbody. Qed.
 
 (* ********************************************************************** *)
 (** Weakening property of [lc_at] *)
@@ -788,19 +520,6 @@ Lemma lc_at_weaken : forall k t,
   term' t -> lc_at k t.
 Proof. introv H. apply~ (@lc_at_weaken_ind 0). omega. Qed.
 
-
-(* ********************************************************************** *)
-(** Weakening property of [Llc_at] *)
-
-Lemma Llc_at_weaken_ind : forall k1 k2 t,
-  Llc_at k1 t -> k1 <= k2 -> Llc_at k2 t.
-Proof. introv. gen k1 k2. induction t; simpl; introv T Lt; auto*.
-       omega. apply (IHt (S k1) (S k2)); trivial; try omega.
-Qed. 
-
-Lemma Llc_at_weaken : forall k t,
-  Lterm' t -> Llc_at k t.
-Proof. introv H. apply~ (@Llc_at_weaken_ind 0). omega. Qed.
 
 (* ********************************************************************** *)
 (** pterm lists *)
@@ -1123,14 +842,91 @@ Proof.
   rewrite <- app_assoc. rewrite <- app_assoc; simpl; trivial.
 Qed.  
 
+(* ********************************************************************** *)
+(** About SN & NF **)
 
-(** maybe realocate  end *)
+Lemma NF_to_SN0 : forall R t, NF R t -> SN_ind 0 R t.
+Proof.
+ intros R t H.
+ apply SN_intro.
+ intros t' H'. unfold NF in H.
+ assert (Q : ~ R t t'). apply H.
+ contradiction.
+Qed.
 
+Lemma SN0_to_NF : forall R t, SN_ind 0 R t -> NF R t.
+Proof.
+ intros R t H. unfold NF.
+ intros t' H'. inversion H.
+ case H0 with (t' := t'). assumption.
+ intros n H''. omega.
+Qed.
+
+Lemma NF_eq_SN0 : forall R t, NF R t <-> SN_ind 0 R t.
+Proof. intros R t. split; [apply NF_to_SN0 | apply SN0_to_NF]. Qed.
+
+
+Lemma WSN : forall n k R t, k <= n -> SN_ind k R t -> SN_ind n R t.
+Proof.
+ intros n k R t H.
+ destruct H; trivial. intro H'.
+ apply SN_intro. intros t' H''. destruct H'.
+ case (H0 t'); trivial. intros n' H'''. exists n'.
+ split; try omega. apply H'''.
+Qed.
+
+Lemma SN_one_step : forall n (R : pterm -> pterm -> Prop) t u, R t u -> SN_ind (S n) R t -> SN_ind n R u.
+Proof.
+ intros n R t u H H'. 
+ destruct H'. case (H0 u); trivial.
+ intro n'. intro H'. apply WSN with (k := n'). omega.
+ apply H'.
+Qed.
+
+Lemma SN_trs : forall n R t u, trans_closure R t u -> 
+                               SN_ind n R t -> (exists k, k < n /\ SN_ind k R u).
+Proof.
+ intros. generalize n H0; clear n H0.
+ induction H; intros. destruct n. apply False_ind. apply SN0_to_NF in H0. 
+ apply (H0 u); trivial. apply SN_one_step with (u := u) in H0; trivial. 
+ exists n. split; try omega; trivial.
+ destruct H1. case (H1 u); trivial; clear H1. intros n' H1. destruct H1.
+ case IHtrans_closure with (n := n'); trivial. intros k' H3. destruct H3.
+ exists k'. split; try omega; trivial.
+Qed.
+
+(*** about SN and NF in lists *)
+
+Lemma NF_eq_SN0_list : forall R lt, NF R %% lt <-> SN_ind 0 R %% lt.
+Proof.
+ intros R lt. induction lt; simpl; split; trivial.
+ intro H. destruct H. split. 
+ apply NF_to_SN0; trivial. apply IHlt; trivial.
+ intro H. destruct H. split.
+ apply SN0_to_NF; trivial. apply IHlt; trivial.
+Qed.
+
+Lemma WSN_list : forall n k R lt, k <= n -> SN_ind k R %% lt -> SN_ind n R %% lt.
+Proof.
+ intros n k R lt H. induction lt; simpl; trivial.
+ intro H'. destruct H'. split. apply WSN with (k := k); trivial.
+ apply IHlt; trivial.
+Qed.
+
+Lemma SN_list : forall R lt, SN R %% lt <-> exists n, SN_ind n R %% lt.
+Proof.
+ intros R lt. induction lt; simpl; split; intros; trivial.
+ exists 0; trivial. destruct IHlt. destruct H. case H0; clear H0; trivial.
+ intros n H0. case H; clear H. intros n' H. exists (n + n').
+ split. apply WSN with (k := n'); try omega; trivial.
+ apply WSN_list with (k := n); try omega; trivial. split.
+ case H; clear H. intros n H. destruct H. exists n; trivial.
+ case H; clear H. intros n H. destruct H. apply IHlt. exists n; trivial.
+Qed.
 
 (* ********************************************************************** *)
 (** Induction Principles Part 2 *)
 
-(* A home made induction principle based on the size of the terms *)
 Lemma term_size_induction :
  forall P : pterm -> Prop,
  (forall x, P (pterm_fvar x)) ->
@@ -1245,46 +1041,6 @@ Proof.
      contradiction.
 Qed.
 
-Lemma Lbody_size_induction :
- forall P : pterm -> Prop,
- (P (pterm_bvar 0)) ->
- (forall x, P (pterm_fvar x)) ->
- (forall t1, (Llc_at 2 t1) ->
-    (forall t2 x, x \notin fv t2 -> pterm_size t2 = pterm_size t1 ->
-    Lbody (open_rec 1 (pterm_fvar x) t2) -> P (open_rec 1 (pterm_fvar x) t2)) -> P (pterm_abs t1)) ->
- (forall t1 t2, Lbody t1 -> Lbody t2 -> P t1 -> P t2 -> P (pterm_app t1 t2)) ->
- (forall t, Lbody t -> P t).
-Proof.
-  intros P Ha Hb Hc Hd t.
-  gen_eq n: (pterm_size t). gen t.
-  induction n using peano_induction.
-  introv Eq B. subst. destruct t. 
-     (* bvar *)
-     generalize B; clear B; case n.
-     intro B; apply Ha.
-     intros n' H'; apply not_Lbody_Sn in H'; contradiction.
-     (* fvar *)
-     apply Hb.
-     (* app *)
-     apply~ Hd; 
-     apply Lbody_distribute_over_application in B.
-     apply B. apply B.
-     apply~ H. simpl; omega. 
-     apply B. apply~ H. simpl; omega.
-     apply B.
-     (* abs *)
-     apply* Hc.
-     apply Lbody_to_Lbody' in B.
-     unfold Lbody' in B. simpl in B; trivial.
-     introv Fr Eq.
-     apply~ H. rewrite <- pterm_size_open_var. simpl. omega.
-     (* sub *)
-     apply Lbody_to_Lbody' in B. unfold Lbody' in B. simpl in B.
-     contradiction.
-     (* sub' *)
-     apply Lbody_to_Lbody' in B. unfold Lbody' in B. simpl in B.
-     contradiction.
-Qed.
 
 Lemma term_size_induction2 :
  forall P : pterm -> Prop,
@@ -1341,77 +1097,6 @@ Proof.
  intros; contradiction. 
  simpl. trivial.
 Qed.
-
-(* A home made induction principle based on the size of the terms *)
-Lemma Lterm_size_induction :
- forall P : pterm -> Prop,
- (forall x, P (pterm_fvar x)) ->
- (forall t1 t2,
-    Lterm t1 -> P t1 -> Lterm t2 -> P t2 -> P (pterm_app t1 t2)) ->
- (forall t1,
-    Lbody t1 ->
-    (forall t2 x, x \notin fv t2 -> pterm_size t2 = pterm_size t1 ->
-      Lterm (t2 ^ x) -> P (t2 ^ x)) ->
-    P (pterm_abs t1)) ->
- (forall t, Lterm t -> P t).
-Proof.
-  intros P Ha Hb Hc t.
-  gen_eq n: (pterm_size t). gen t.
-  induction n using peano_induction.
-  introv Eq T. subst. inverts T. 
-     apply Ha.
-     (* app *)
-     apply~ Hb. apply~ H. simpl; omega. apply~ H. simpl; omega.
-     (* abs *)
-     apply* Hc.
-       introv. exists L. trivial.
-       introv Fr Eq T.
-       apply~ H. unfold open.
-      rewrite <- pterm_size_open_var. simpl. omega.
- Qed.
-
-Lemma Lterm_size_induction2 :
- forall P : pterm -> Prop,
- (forall x l, (forall u, In u l -> (Lterm u /\ P u)) -> P ((pterm_fvar x) // l)) ->
- (forall t1 l, (forall u, In u l -> (Lterm u /\ P u)) -> Lbody t1 ->
-  (forall t2 x, x \notin fv t2 -> pterm_size t2 = pterm_size t1 -> Lterm (t2 ^ x) -> P (t2 ^ x)) ->
-      P ((pterm_abs t1) // l)) ->
- (forall l t, (forall u, In u l -> (Lterm u /\ P u)) -> Lterm t -> P (t // l)).
-Proof.
- intros. generalize H2.  intro T. generalize l H1 H2. clear l H1 H2.
- apply Lterm_size_induction with (t := t); trivial; intros.
- apply H; trivial.
- replace (pterm_app t1 t2 // l) with (t1 // l ++ (t2 :: nil)).  
- apply H2. intros. apply in_app_iff in H7. destruct H7.
- apply H5; trivial. simpl in H7. destruct H7; try contradiction.
- rewrite <- H7. clear H7. inversion H6. split; trivial.
- assert (Q : P (t2 // nil)). 
-   apply H4; simpl; trivial; intros. contradiction. 
- simpl in Q. trivial. trivial. 
- rewrite mult_app_append. trivial.
- apply H0; trivial. intros.
- assert (Q : P (t2 ^ x // nil)).
-   apply H2; simpl; trivial; intros. contradiction.
- simpl in Q. trivial.
-Qed.
-
-
-Lemma Lterm_size_induction3 :
- forall P : pterm -> Prop,
- (forall x l, (forall u, In u l -> (Lterm u /\ P u)) -> P ((pterm_fvar x) // l)) ->
- (forall t1 l, (forall u, In u l -> (Lterm u /\ P u)) -> Lbody t1 ->
-  (forall t2 x, x \notin fv t2 -> pterm_size t2 = pterm_size t1 -> Lterm (t2 ^ x) -> P (t2 ^ x)) ->
-      P ((pterm_abs t1) // l)) ->
- (forall t, Lterm t -> P t).
-Proof. 
- intros. replace t with (t // nil).
- apply Lterm_size_induction2; simpl; trivial.
- intros; contradiction. 
- simpl. trivial.
-Qed.
-
-
-
 
 (* ******************************* *)
 (** * Tactics depending on lemmas  *)
@@ -1534,8 +1219,8 @@ Proof.
   intros. rewrite swap_sym. apply swap_var_l.
 Qed.
 
-Lemma swap_eq_subst : forall (x y z : var) t, z <> x -> z <> y -> z \notin (fv t) ->  
-      subst z (pterm_fvar y) ((subst y (pterm_fvar x) (subst x (pterm_fvar z) t))) = [(x,y)] t.
+Lemma swap_eq_m_sb : forall (x y z : var) t, z <> x -> z <> y -> z \notin (fv t) ->  
+      m_sb z (pterm_fvar y) ((m_sb y (pterm_fvar x) (m_sb x (pterm_fvar z) t))) = [(x,y)] t.
 Proof.
  intros. induction t.
  simpl; trivial. simpl in H. apply notin_singleton in H1.
@@ -1579,7 +1264,7 @@ Proof.
  intro H1. pick_fresh z. 
  apply notin_union in Fr. destruct Fr. apply notin_union in H2. destruct H2.
  apply notin_singleton in H2. apply notin_singleton in H4.
- rewrite <- swap_eq_subst with (z := z); trivial.
+ rewrite <- swap_eq_m_sb with (z := z); trivial.
  repeat rewrite subst_open_gen; trivial.  
  replace  ([z ~> pterm_fvar y]([y ~> pterm_fvar x]([x ~> pterm_fvar z]t))) with t.
  replace ([x ~> pterm_fvar z]pterm_fvar y) with (pterm_fvar y).
@@ -2056,33 +1741,7 @@ Proof.
  intros n k H0 H1. simpl in *|-*. contradiction.
 Qed.
  
-Lemma Llc_at_bswap : forall n k t, S k < n -> Llc_at n t -> Llc_at n (bswap_rec k t).
-Proof.
- intros n k t. 
- generalize n k; clear n k.
- induction t.
- (* bvar *)
- intros n' k H0 H1. simpl in H1.
- unfolds bswap_rec. 
- case (k === n). intro H2.
- rewrite H2. simpl. omega. intro H2.
- case (S k === n). intro H3. simpl. omega. intro H3. 
- simpl. trivial.
- (* fvar *)
- intros n k H0 H1. simpl in *|-*. trivial.
- (* app *)
- intros n k H0 H1. simpl in *|-*. destruct H1. split.
- apply IHt1; trivial. apply IHt2; trivial.
- (* abs *)
- intros n k H0 H1. simpl in *|-*.
- apply IHt; try omega; trivial.
- (* sub *)
- intros n k H0 H1. simpl in *|-*. contradiction. 
- (* sub' *)
- intros n k H0 H1. simpl in *|-*. contradiction. 
-Qed.
 
- 
 Lemma lc_at_open : forall n t u, term u -> (lc_at (S n) t <-> lc_at n (open_rec n u t)).
 Proof.
  intros n t u T. split.
@@ -2139,55 +1798,6 @@ Proof.
  simpl. intros. contradiction.
 Qed.
 
-Lemma Llc_at_open : forall n t u, Lterm u -> (Llc_at (S n) t <-> Llc_at n (open_rec n u t)).
-Proof.
- intros n t u T. split.
-(* -> *)
- generalize n; clear n.
- induction t.
- (* bvar *)
- intros n' H0. unfolds open_rec.
- case (n' === n). intro H1.
- rewrite H1 in H0. rewrite H1. simpl in *|-*. 
- apply Lterm_to_Lterm' in T. unfold Lterm' in T.
- apply Llc_at_weaken_ind with (k1 := 0); try omega; trivial.
- intro H1. simpl in *|-*. omega.
- (* fvar *)
- intros n H. simpl. trivial.
- (* app *)
- intros n H. simpl in *|-*.
- case H; clear H; intros Ht1 Ht2; split.
- apply (IHt1 n Ht1). 
- apply (IHt2 n Ht2).
- (* abs *)
- intros n H. simpl in *|-*.
- apply (IHt (S n) H).
- (* sub *)
- intros n H. simpl in *|-*. contradiction.
- (* sub' *)
- intros n H. simpl in *|-*. contradiction.
-(* <- *)
- generalize n; clear n.
- induction t.
- (* bvar *)
- intros n' H0. simpl in H0.
- case (n' === n) in H0. simpl. omega.
- simpl in *|-*. omega.
- (* fvar *)
- simpl. trivial. 
- (* app *)
- simpl in *|-*. intros n H.
- case H; clear H; intros Ht1 Ht2; split.
- apply (IHt1 n Ht1). 
- apply (IHt2 n Ht2).
- (* abs *)
- simpl in *|-*. intros n H. 
- apply (IHt (S n) H).
- (* sub *)
- simpl in *|-*. intros n H. contradiction. 
- (* sub' *)
- simpl in *|-*. intros n H. contradiction.
-Qed.
 
 
 Lemma lc_at_open' : forall n k t u, term u -> k < n -> (lc_at n (open_rec k u t) <-> lc_at n t).
@@ -2383,3 +1993,856 @@ Proof.
  try omega; trivial.
 Qed.
 
+(*
+Lemma open_rec_indep_comm: forall t x y, {0 ~> pterm_fvar x}({1 ~> pterm_fvar y}t) = {1 ~> pterm_fvar y}({0 ~> pterm_fvar x}t). 
+Proof.
+  Admitted.*)
+    
+Lemma lc_at_open_rec_rename: forall t x y m n, lc_at m (open_rec n (pterm_fvar x) t) -> lc_at m (open_rec n (pterm_fvar y) t).
+Proof.
+  induction t. simpl. introv H. case_nat. constructor. assumption.
+  simpl. intros; trivial. simpl. introv H. destruct H.
+  apply (IHt1 x y) in H. apply (IHt2 x y) in H0.
+  split; assumption. simpl.
+  introv H. apply IHt with x. assumption. simpl.
+  introv H. destruct H. split. apply IHt1 with x; assumption. apply IHt2 with x; assumption.
+  simpl. trivial.
+Qed.  
+
+Corollary term_open_rename: forall t x y, term (t^x) -> term (t^y).  
+Proof.
+  introv H. apply term_eq_term' in H. apply term_eq_term'.
+  apply lc_at_open_rec_rename with x. assumption.
+Qed.
+  
+Lemma body_to_term: forall t x, x \notin fv t -> body t -> term (t^x).
+Proof.
+  intros. inversion* H0.
+Qed.
+
+Lemma term_to_body: forall t x, x \notin fv t -> term (t^x) -> body t.
+Proof.
+  introv H H'. 
+  unfold body.
+  exists (fv t). introv H''. apply term_open_rename with x; assumption.
+Qed.
+  
+(* ********************************************************************** *)
+(** Properties of reduction *)
+
+Definition red_regular (R : pterm -> pterm -> Prop) :=
+  forall t t', R t t' -> term t /\ term t'.
+
+Definition red_regular' (R : pterm -> pterm -> Prop) :=
+  forall t t', R t t' -> (term t <-> term t').
+
+Definition red_refl (R : pterm -> pterm -> Prop) :=
+  forall t, term t -> R t t.
+
+Definition red_in (R : pterm -> pterm -> Prop) :=
+  forall t x u u', term t -> R u u' ->
+  R ([x ~> u]t) ([x ~> u']t).
+ 
+Definition red_all (R : pterm -> pterm -> Prop) :=
+  forall x t t', R t t' -> 
+  forall u u', R u u' -> 
+  R ([x~>u]t) ([x~>u']t').
+
+Definition red_out (R : pterm -> pterm -> Prop) :=
+  forall x u t t', term u -> R t t' -> 
+  R ([x~>u]t) ([x~>u]t').
+
+Definition red_out' (R : pterm -> pterm -> Prop) :=
+  forall x y t t', R t t' -> 
+  R ([x~>pterm_fvar y]t) ([x~>pterm_fvar y]t').
+
+Definition red_rename (R : pterm -> pterm -> Prop) :=
+  forall x t t' y,
+  x \notin (fv t) -> x \notin (fv t') ->
+  R (t ^ x) (t' ^ x) -> 
+  R (t ^ y) (t' ^ y).
+
+Definition red_rename' (R : pterm -> pterm -> Prop) :=
+  forall x t t' y,
+  x \notin (fv t) -> x \notin (fv t') ->
+  y \notin (fv t) -> y \notin (fv t') ->
+  R (t ^ x) (t' ^ x) -> 
+  R (t ^ y) (t' ^ y).
+
+Definition red_swap (R : pterm -> pterm -> Prop) :=
+  forall x t t' y,
+  R t t' ->
+  R ([(x,y)]t) ([(x,y)]t').
+
+Definition red_through (R : pterm -> pterm -> Prop) :=
+  forall x t1 t2 u1 u2, 
+  x \notin (fv t1) -> x \notin (fv u1) ->
+  R (t1 ^ x) (u1 ^ x) -> R t2 u2 ->
+  R (t1 ^^ t2) (u1 ^^ u2).
+
+Definition red_not_fv (R: pterm -> pterm -> Prop) :=
+  forall x t t', R t t' ->
+  x \notin (fv t) -> x \notin (fv t'). 
+
+Definition red_fv (R: pterm -> pterm -> Prop) :=
+  forall x t t', R t t' ->
+  x \in (fv t') -> x \in (fv t). 
+
+Lemma red_regular_ctx: forall (R : pterm -> pterm -> Prop),
+  red_regular R -> red_regular (ES_contextual_closure R).
+ Proof.
+  intros_all. induction H0.
+  apply H; trivial. 
+  case IHES_contextual_closure; clear IHES_contextual_closure.
+  intros H2 H3. split; apply term_distribute_over_application; split ; trivial.
+  case IHES_contextual_closure; clear IHES_contextual_closure.
+  intros H2 H3. split; apply term_distribute_over_application; split ; trivial.
+  split; apply body_to_term_abs; unfold body; exists L;
+  intros; apply H1; trivial.
+  split; apply body_to_subs; trivial; unfold body; exists L; intros; apply H1; trivial.
+  split; apply body_to_subs; apply term_is_a_body in H1.
+  assumption. apply IHES_contextual_closure. 
+  assumption. apply IHES_contextual_closure. 
+Qed.
+
+ (** flavio 2016/02/19
+Lemma SN_app : forall n R t u, red_regular R ->  
+               SN_ind n (ES_contextual_closure R) (pterm_app t u) ->
+               SN_ind n (ES_contextual_closure R) t /\ SN_ind n (ES_contextual_closure R) u.
+Proof.
+ intros n R t u Reg. 
+ generalize dependent u.
+ generalize dependent t.
+ induction n.  intros t u H. split; rewrite <- NF_eq_SN0 in *; unfold NF in *. 
+ intros t' H'. apply (H (pterm_app t' u)).
+ apply ES_app_left. assumption.
+ false_goal.
+ assert (ES_contextual_closure R (pterm_app t u) (pterm_app t' u)).
+ apply ES_app_left; trivial. 
+ intros u' H'. apply (H (pterm_app t u')). apply ES_app_right; trivial.
+ intros t u H. destruct H. split. 
+ apply SN_intro. intros t' H'. exists n. split; try omega. 
+ apply IHn with (t := t') (u := u); trivial. apply red_regular_ctx in Reg.
+ apply Reg in H'. apply H'. case (H (pterm_app t' u)). apply app_left; trivial. 
+ intros k H''. apply WSN with (k := k). omega. apply H''.
+ apply SN_intro. intros u' H'. exists n. split; try omega. 
+ apply IHn with (t := t) (u := u'); trivial. apply red_regular_ctx in Reg.
+ apply Reg in H'. apply H'. case (H (pterm_app t u')). apply app_right; trivial. 
+ intros k H''. apply WSN with (k := k). omega. apply H''.
+Qed. 
+
+
+Lemma SN_abs : forall x n R t, red_regular R -> red_out R -> 
+               SN_ind n (contextual_closure R) (pterm_abs t) ->
+               x \notin (fv t) -> SN_ind n (contextual_closure R) (t ^ x).
+Proof.
+ intros x n R t Reg Out.
+ generalize t; clear t.
+ apply red_regular_ctx in Reg. gg
+ apply red_out_ctx in Out. 
+ apply red_out_to_rename in Out.
+ induction n. intros. 
+ apply SN0_to_NF in H. 
+ apply NF_to_SN0; unfold NF in *|-*.
+ intros t' H'. gen_eq t0 : (close t' x). intro H1.
+ replace t' with (t0 ^ x) in H'.
+ assert (Q: contextual_closure R (pterm_abs t) (pterm_abs t0)).
+    apply abs_in with (L := {{x}}). intros z H2. 
+    apply notin_singleton in H2. apply Out with (x := x); trivial.
+    rewrite H1. apply fv_close'.
+ assert (Q': ~ contextual_closure R (pterm_abs t) (pterm_abs t0)).
+    apply H.
+ contradiction. rewrite H1. rewrite open_close_var with (x := x).
+ reflexivity. apply Reg in H'. apply H'.
+ intros. destruct H. apply SN_intro.
+ intros. exists n. split; try omega.
+ gen_eq t0 : (close t' x). intro H2.
+ replace t' with (t0 ^ x). replace t' with (t0 ^ x) in H1.
+ apply IHn; trivial. case (H (pterm_abs t0)); trivial.
+ apply abs_in with (L := {{x}}).
+ intros z H3. apply notin_singleton in H3. 
+ apply Out with (x := x); trivial.
+ rewrite H2. apply fv_close'.
+ intros k H3. apply WSN with (k := k); try omega.
+ apply H3. rewrite H2. apply fv_close'.
+ rewrite H2. rewrite open_close_var with (x := x).
+ reflexivity. apply Reg in H1. apply H1.
+ rewrite H2. rewrite open_close_var with (x := x).
+ reflexivity. apply Reg in H1. apply H1. 
+Qed.
+
+
+Lemma SN_sub : forall x n R t u, red_regular R -> red_out R -> 
+               body t -> term u -> x \notin (fv t) -> 
+               SN_ind n (contextual_closure R) (t[u]) ->
+               SN_ind n (contextual_closure R) (t ^ x) /\
+               SN_ind n (contextual_closure R) u.
+Proof.
+ intros x n R t u Reg Out.
+ generalize t u; clear t u.
+ apply red_regular_ctx in Reg. 
+ apply red_out_ctx in Out. 
+ apply red_out_to_rename in Out.
+ induction n. intros. 
+ apply SN0_to_NF in H2. split; intros;
+ apply NF_to_SN0; unfold NF in *|-*.
+ intros t' H'. gen_eq t0 : (close t' x). intro H3.
+ replace t' with (t0 ^ x) in H'.
+ assert (Q: contextual_closure R (t[u])(t0[u])).
+    apply subst_left with (L := {{x}}); trivial. intros z H4. 
+    apply notin_singleton in H4. apply Out with (x := x); trivial.
+    rewrite H3. apply fv_close'.
+ assert (Q': ~ contextual_closure R (t[u]) (t0[u])).
+    apply H2.
+ contradiction. rewrite H3. rewrite open_close_var with (x := x).
+ reflexivity. apply Reg in H'. apply H'.
+ intros t' H'.
+ assert (Q: contextual_closure R (t[u])(t[t'])).
+   apply subst_right; trivial. 
+ assert (Q': ~ contextual_closure R (t[u])(t[t'])).
+   apply H2.
+ contradiction.
+ intros. destruct H2. split. intros. apply SN_intro.
+ intros. exists n. split; try omega.
+ gen_eq t0 : (close t' x). intro H4.
+ replace t' with (t0 ^ x). replace t' with (t0 ^ x) in H3.
+ assert (Q : x \notin fv t0). rewrite H4. apply fv_close'.
+ apply (IHn t0 u); trivial. apply Reg in H3.
+ apply body'_to_body. case H3; clear H3. intros H3 H5.
+ apply term_to_term' in H5. unfold body'. unfold term' in H5.
+ unfold open in H5. apply lc_at_open in H5; trivial.
+ case (H2 (t0[u])); trivial.
+ apply subst_left with (L := {{x}}); trivial.
+ intros z H5. apply notin_singleton in H5. 
+ apply Out with (x := x); trivial.
+ intros k H5. apply WSN with (k := k); try omega. apply H5.
+ rewrite H4. rewrite open_close_var with (x := x).
+ reflexivity. apply Reg in H3. apply H3.
+ rewrite H4. rewrite open_close_var with (x := x).
+ reflexivity. apply Reg in H3. apply H3.
+ apply SN_intro.
+ intros t' H'. exists n.
+ split; try omega. 
+ apply IHn with (t := t) (u := t'); trivial.
+ apply Reg in H'. apply H'.
+ case (H2 (t[t'])).
+ apply subst_right; trivial. 
+ intros k H''. apply WSN with (k := k).
+ omega. apply H''.
+Qed.
+
+Lemma SN_mult_app : forall n R t l, red_regular R ->  term t -> term %% l -> 
+               SN_ind n (contextual_closure R) (t // l) ->
+               SN_ind n (contextual_closure R) t /\ SN_ind n (contextual_closure R) %% l.
+Proof.
+ intros n R t l Reg. generalize n t; clear n t.
+ induction l; simpl. intros n t T H0 H. split; trivial.
+ intros n t T H0 H. destruct H0. apply SN_app in H; trivial. destruct H.
+ assert (Q : SN_ind n (contextual_closure R) t /\ SN_ind n (contextual_closure R) %% l). 
+  apply IHl; trivial.
+ clear IHl. destruct Q. split; trivial. split; trivial.
+ rewrite term_mult_app. split; trivial. 
+Qed. 
+*)
+
+
+(** Reduction on lists **)
+
+Definition R_list (R : pterm -> pterm -> Prop) (l : list pterm) (l' : list pterm) := 
+exists t, exists t', exists l0, exists l1, l = (l0 ++ t :: l1) /\ l' = (l0 ++ t' :: l1) /\ R t t'.
+
+Lemma R_list_h: forall (R : pterm -> pterm -> Prop) a b lt, 
+                R a b -> R_list R (a :: lt) (b :: lt).   
+Proof.
+ intros. unfold R_list. exists a. exists b. exists (nil (A := pterm)). exists lt.
+ simpl. split; trivial; split; trivial.
+Qed.
+
+Lemma R_list_t: forall (R : pterm -> pterm -> Prop) a lt lt', 
+                (R_list R lt lt') -> R_list R (a :: lt) (a :: lt').
+Proof.
+ unfold R_list. intros.
+ case H; clear H. intros b H.
+ case H; clear H. intros b' H.
+ case H; clear H. intros l H.
+ case H; clear H. intros l' H.
+ destruct H. destruct H0. 
+ rewrite H. rewrite H0.
+ exists b. exists b'. 
+ exists (a :: l). exists l'. simpl.
+ split; trivial. split; trivial.
+Qed.
+
+Lemma term_mult_app : forall t lu, term (t // lu) <-> term t /\ (term %% lu).
+Proof.
+ intros t lu. induction lu; simpl; split; 
+ intro H;  try apply H; try split; trivial.
+ apply term_distribute_over_application in H. 
+ apply IHlu. apply H.
+ apply term_distribute_over_application in H.
+ split. apply H. apply IHlu. apply H.
+ apply term_distribute_over_application. split.
+ apply IHlu. split; apply H. apply H.
+Qed.
+
+Lemma ctx_red_t_mult_app : forall R t lu lu', term t -> term %% lu -> R_list (ES_contextual_closure R) lu lu' -> (ES_contextual_closure R) (t // lu) (t // lu').
+Proof.
+ intros R t lu lu' Tt Tlu H. unfold R_list in H. 
+ case H; clear H; intros t0 H.
+ case H; clear H; intros t1 H.
+ case H; clear H; intros l0 H.
+ case H; clear H; intros l1 H.
+ destruct H. destruct H0. 
+ rewrite H. rewrite H0. rewrite H in Tlu. 
+ clear H H0. induction l0; simpl. destruct l1; simpl. 
+ apply ES_app_right; trivial.
+ apply ES_app_right; trivial. 
+ simpl in Tlu. rewrite term_distribute_over_application.
+ rewrite term_mult_app. destruct Tlu. destruct H0.
+ split; trivial. split; trivial.
+ simpl in Tlu. destruct Tlu. 
+ apply ES_app_left; trivial.
+ apply IHl0; trivial. 
+Qed.
+
+Lemma contextual_R1_R2: forall (R1 R2: pterm -> pterm -> Prop), 
+                           (forall t t', R1 t t' -> R2 t t') -> 
+                           (forall t t', ES_contextual_closure R1 t t' -> ES_contextual_closure R2 t t').
+Proof.
+ intros R1 R2 H t t' H'. induction H'.
+ apply ES_redex. apply H; trivial.
+ apply ES_app_left; trivial.
+ apply ES_app_right; trivial.
+ apply ES_abs_in with (L := L); trivial.
+ apply ES_subst_left with (L := L); trivial.
+ apply ES_subst_right; trivial.
+Qed.
+
+Lemma ctx_red_h_mult_app : forall R t t' lu, term %% lu -> (ES_contextual_closure R) t t' -> (ES_contextual_closure R) (t // lu) (t' // lu).
+Proof.
+ intros R t t' lu Tlu H. induction lu; simpl in *|-*; trivial.
+ destruct Tlu. apply ES_app_left; trivial.
+ apply IHlu; trivial.
+Qed.
+
+(* ********************************************************************** *)
+(** Some relations between the properties of relations *)
+
+Lemma red_all_to_out : forall (R : pterm -> pterm -> Prop), 
+  red_all R -> red_refl R -> red_out R. 
+Proof.
+  intros_all. auto*.
+Qed.
+
+Lemma red_out_to_out' : forall (R : pterm -> pterm -> Prop),
+  red_out R -> red_out' R. 
+Proof.
+ intros_all. apply H; trivial.
+Qed.
+
+Lemma red_out'_to_rename : forall (R : pterm -> pterm -> Prop),
+  red_out' R -> red_rename R. 
+Proof.
+  intros_all.
+  rewrite* (@subst_intro x t). 
+  rewrite* (@subst_intro x t').
+Qed.
+
+Lemma red_out_to_rename : forall (R : pterm -> pterm -> Prop),
+  red_out R -> red_rename R.
+Proof.
+  intros. apply red_out'_to_rename. 
+  apply red_out_to_out'; trivial.
+Qed.
+
+
+Lemma red_all_to_through : forall (R : pterm -> pterm -> Prop),
+  red_regular R -> red_all R -> red_through R. 
+Proof.
+  intros_all. lets: (H _ _ H4).
+  rewrite* (@subst_intro x t1). 
+  rewrite* (@subst_intro x u1).
+Qed.
+
+Lemma red_out_to_swap : forall (R : pterm -> pterm -> Prop),
+  red_out R -> red_swap R. 
+Proof.
+  intros_all. pick_fresh z.
+  apply notin_union in Fr; destruct Fr.
+  apply notin_union in H1; destruct H1.
+  apply notin_union in H1; destruct H1.
+  apply notin_singleton in H1.
+  apply notin_singleton in H4.
+  repeat rewrite <- swap_eq_m_sb with (z := z); trivial.
+  repeat apply H; trivial.
+Qed. 
+
+Lemma red_rename_to_rename' : forall (R : pterm -> pterm -> Prop),
+  red_rename R -> red_rename' R. Print red_rename'.
+Proof.
+ intros_all. apply H with (x := x); trivial.
+Qed.
+
+Lemma red_swap_to_rename' : forall (R : pterm -> pterm -> Prop),
+  red_swap R -> red_rename' R.
+Proof.
+  intros_all. unfold red_swap in H.
+  case (x == y); intro H'. rewrite <- H'; trivial.
+  apply (H x (t ^ x) (t' ^ x) y) in H4. unfold open in *|-*.
+  rewrite open_swap_comm in H4.  rewrite open_swap_comm in H4.
+  simpl in H4. case (x == y); case (x == x) in H4; intros; try contradiction. clear e n. 
+  rewrite swap_fresh in H4; trivial. rewrite swap_fresh in H4; trivial.  
+  apply False_ind. apply n; trivial.
+Qed.
+
+Lemma red_out'_to_swap : forall (R : pterm -> pterm -> Prop),
+  red_out' R -> red_swap R.
+Proof. 
+  intros_all. pick_fresh z.
+  apply notin_union in Fr; destruct Fr.
+  apply notin_union in H1; destruct H1.
+  apply notin_union in H1; destruct H1.
+  apply notin_singleton in H1.
+  apply notin_singleton in H4.
+  repeat rewrite <- swap_eq_m_sb with (z := z); trivial.
+  repeat apply H; trivial.
+Qed. 
+
+(** flavio 2016/02/19
+ Lemma red_regular'_pctx : forall (R : pterm -> pterm -> Prop),
+  red_regular' R -> red_regular' (p_contextual_closure R).
+Proof.
+  intros_all. induction H0.
+  apply H; trivial. 
+  split. intro H1.
+  apply term_distribute_over_application.
+  apply term_distribute_over_application in H1. 
+  destruct H1. split.
+  apply IHp_contextual_closure1; trivial. 
+  apply IHp_contextual_closure2; trivial. 
+  intro H1.
+  apply term_distribute_over_application.
+  apply term_distribute_over_application in H1. 
+  destruct H1. split.
+  apply IHp_contextual_closure1; trivial. 
+  apply IHp_contextual_closure2; trivial. 
+  split. intro H2. 
+  apply body_to_term_abs. apply term_abs_to_body in H2.
+  unfold body. exists (L \u (fv t)). intros x Fr.
+  apply notin_union in Fr. destruct Fr. apply (H1 x); trivial.
+  apply body_to_term; trivial.
+  intro H2. 
+  apply body_to_term_abs. apply term_abs_to_body in H2.
+  unfold body. exists (L \u (fv t')). intros x Fr.
+  apply notin_union in Fr. destruct Fr. apply (H1 x); trivial.
+  apply body_to_term; trivial.
+  split. intro H3. apply subs_to_body in H3. destruct H3.
+  apply body_to_subs. unfold body. exists (L \u (fv t)). intros x Fr.
+  apply notin_union in Fr. destruct Fr. apply (H1 x); trivial.
+  apply body_to_term; trivial. apply IHp_contextual_closure; trivial.
+  intro H3. apply subs_to_body in H3. destruct H3.
+  apply body_to_subs. unfold body. exists (L \u (fv t')). intros x Fr.
+  apply notin_union in Fr. destruct Fr. apply (H1 x); trivial.
+  apply body_to_term; trivial. apply IHp_contextual_closure; trivial.
+Qed.
+
+
+Lemma red_regular_trs : forall (R : pterm -> pterm -> Prop),
+  red_regular R -> red_regular (trans_closure R).
+Proof.
+ intros_all. induction H0.
+ apply H; trivial. 
+ apply H in H0. split; 
+ [apply H0 | apply IHtrans_closure].
+Qed. 
+
+Lemma red_regular'_trs : forall (R : pterm -> pterm -> Prop),
+  red_regular' R -> red_regular' (trans_closure R).
+Proof.
+ intros_all. induction H0.
+ apply H; trivial. 
+ apply H in H0. split.
+ intro. apply IHtrans_closure. apply H0. trivial.
+ intro. apply H0. apply IHtrans_closure. trivial.
+Qed. 
+
+Lemma red_out_ctx : forall (R : pterm -> pterm -> Prop),
+  red_out R -> red_out (contextual_closure R).
+Proof.
+ intros_all. induction H1.
+ apply redex. apply H; trivial.
+ simpl. apply app_left; trivial.
+ apply term'_to_term.
+ unfold term'. apply lc_at_subst;
+ apply term_to_term'; trivial.
+ simpl. apply app_right; trivial.
+ apply term'_to_term.
+ unfold term'. apply lc_at_subst;
+ apply term_to_term'; trivial.
+ simpl. apply abs_in with (L := L \u {{x}}). 
+ intros x0 Fr. apply notin_union in Fr. case Fr. 
+ clear Fr. intros H3 H4.
+ apply notin_singleton in H4.
+ rewrite subst_open_var; trivial.
+ rewrite subst_open_var; trivial.
+ apply H2; trivial.
+ simpl. apply subst_left with (L := L \u {{x}}). 
+ apply term'_to_term.
+ unfold term'. apply lc_at_subst;
+ apply term_to_term'; trivial.
+ intros x0 Fr. apply notin_union in Fr. case Fr. 
+ clear Fr. intros H4 H5.
+ apply notin_singleton in H5.
+ rewrite subst_open_var; trivial.
+ rewrite subst_open_var; trivial.
+ apply H3; trivial.
+ simpl. apply subst_right; trivial.
+ apply body'_to_body.
+ unfold body'. apply lc_at_subst.
+ apply body_to_body'; trivial.
+ apply term_to_term' in H0. unfold term' in H0.
+ apply lc_at_weaken_ind with (k1 := 0); trivial; omega.
+Qed.
+
+Lemma red_out_pctx : forall (R : pterm -> pterm -> Prop),
+  red_out R -> red_out (p_contextual_closure R).
+Proof.
+ intros_all. induction H1; simpl.
+ apply p_redex. apply H; trivial.
+ apply p_app; trivial.
+ apply p_abs_in with (L := L \u {{x}}). 
+ intros x0 Fr. apply notin_union in Fr. destruct Fr. 
+ apply notin_singleton in H4.
+ rewrite subst_open_var; trivial.
+ rewrite subst_open_var; trivial.
+ apply H2; trivial.
+ apply p_subst with (L := L \u {{x}}); trivial.
+ intros x0 Fr. apply notin_union in Fr. destruct Fr. 
+ apply notin_singleton in H5.
+ rewrite subst_open_var; trivial.
+ rewrite subst_open_var; trivial.
+ apply H2; trivial.
+Qed.
+
+Lemma red_out_trs : forall (R : pterm -> pterm -> Prop),
+  red_out R -> red_out (trans_closure R).
+Proof.
+ intros_all. induction H1.
+ apply one_step_reduction. apply H; trivial.
+ apply transitive_reduction with (u := [x ~> u]u0); trivial.
+ apply H; trivial.
+Qed.
+ 
+Lemma red_not_fv_ctx : forall (R : pterm -> pterm -> Prop),
+  red_not_fv R -> red_not_fv (contextual_closure R).
+Proof.
+ intros R H. unfold red_not_fv in *|-*.
+ intros x t t' H'. induction H'.
+ apply H; trivial. 
+ simpl. intro H1.
+ apply notin_union. apply notin_union in H1.
+ split. apply IHH'. apply H1. apply H1.
+ simpl. intro H1.
+ apply notin_union. apply notin_union in H1.
+ split. apply H1. apply IHH'. apply H1.
+ simpl. intro H2. case var_fresh with (L := {{x}} \u L).
+ intros z Fr. apply notin_union in Fr. case Fr; clear Fr.
+ intros H3 H4. apply notin_singleton in H3.
+ apply fv_notin_open with (z := z); auto. apply H1; trivial.
+ apply fv_notin_open; auto.
+ simpl. intro H3.
+ apply notin_union. apply notin_union in H3.
+ split. case var_fresh with (L := {{x}} \u L).
+ intros z Fr. apply notin_union in Fr. case Fr; clear Fr.
+ intros H4 H5. apply notin_singleton in H4.
+ apply fv_notin_open with (z := z); auto. apply H2; trivial.
+ apply fv_notin_open; auto. apply H3. apply H3.
+ simpl. intro H1.
+ apply notin_union. apply notin_union in H1.
+ split. apply H1. apply IHH'. apply H1.
+Qed.
+
+Lemma red_fv_ctx : forall (R : pterm -> pterm -> Prop),
+  red_fv R -> red_fv (contextual_closure R).
+Proof.
+ intros R H. unfold red_not_fv in *|-*.
+ intros x t t' H'. induction H'; simpl.
+ apply H; trivial. intro H1.
+ apply in_union. apply in_union in H1.
+ case H1; clear H1; intro H1. 
+ left. apply IHH'; trivial. right; trivial. intro H1.
+ apply in_union. apply in_union in H1.
+ case H1; clear H1; intro H1.
+ left; trivial. right; apply IHH'; trivial. intro H2.
+ case var_fresh with (L := {{x}} \u L). intros z Fr.
+ apply notin_union in Fr. case Fr; clear Fr; intros H3 H4.
+ apply notin_singleton in H3. apply fv_open_in_neq with (y := z); auto.
+ apply H1; trivial. apply fv_open_in_neq with (y := z); auto.
+ intro H3. apply in_union. apply in_union in H3.
+ case H3; clear H3; intro H3. left.
+ case var_fresh with (L := {{x}} \u L). intros z Fr.
+ apply notin_union in Fr. case Fr; clear Fr; intros H4 H5.
+ apply notin_singleton in H4. apply fv_open_in_neq with (y := z); auto.
+ apply H2; trivial. apply fv_open_in_neq with (y := z); auto. right; trivial.
+ intro H1. apply in_union. apply in_union in H1.
+ case H1; clear H1; intro H1. left; trivial. right; apply IHH'; trivial.  
+Qed.
+
+Lemma red_swap_ctx: forall (R : pterm -> pterm -> Prop),
+  red_swap R -> red_swap (contextual_closure R).
+Proof.
+ intros R H. unfold red_swap in *|-*.
+ intros x t t' y H'. induction H'; simpl.
+ apply redex. apply H; trivial.
+ apply app_left; trivial. apply swap_term; trivial.
+ apply app_right; trivial. apply swap_term; trivial.
+ apply abs_in with (L := L \u {{x}} \u {{y}}). intros z Hz.
+ apply notin_union in Hz; destruct Hz.
+ apply notin_union in H2; destruct H2.
+ apply notin_singleton in H3. apply notin_singleton in H4.
+ rewrite open_swap; trivial. rewrite open_swap; trivial.
+ apply H1; trivial.
+ apply subst_left with (L := L \u {{x}} \u {{y}}). apply swap_term; trivial.
+ intros z Hz.
+ apply notin_union in Hz; destruct Hz.
+ apply notin_union in H3; destruct H3.
+ apply notin_singleton in H4. apply notin_singleton in H5.
+ rewrite open_swap; trivial. rewrite open_swap; trivial.
+ apply H2; trivial.
+ apply subst_right; trivial. 
+ inversion H0. clear H0. exists (x0 \u {{x}} \u {{y}}). intros z Hz.
+ apply notin_union in Hz; destruct Hz.
+ apply notin_union in H0; destruct H0.
+ apply notin_singleton in H2. apply notin_singleton in H3.
+ rewrite open_swap; trivial. apply swap_term. apply H1; trivial.
+Qed.
+ 
+Lemma red_swap_trs: forall (R : pterm -> pterm -> Prop),
+  red_swap R -> red_swap (trans_closure R).
+Proof.
+ intros R H. unfold red_swap in *|-*. intros x t t' y H'.
+ induction H'. apply one_step_reduction. apply H; trivial.
+ apply transitive_reduction with (u := ([(x,y)]u)); trivial.
+ apply H; trivial.
+Qed.
+
+Lemma ctx_abs_in_close : forall x R L t t', red_regular R -> red_out R ->
+                        contextual_closure R t t' -> x \notin L ->
+                        contextual_closure R (pterm_abs (close t x)) (pterm_abs (close t' x)).
+Proof.
+ intros x R L t t' H0 H1 H2 Fr.
+ apply abs_in with (L := L). intros z Fr'. 
+ apply red_out_ctx in H1. apply red_out_to_rename in H1.
+ apply H1 with (x := x). apply fv_close'. apply fv_close'.
+ replace (close t x ^ x) with t. replace (close t' x ^ x) with t'; trivial.
+ apply open_close_var. apply red_regular_ctx in H0. apply H0 in H2. apply H2.
+ apply open_close_var. apply red_regular_ctx in H0. apply H0 in H2. apply H2.
+Qed.
+
+Lemma pctx_abs_in_close : forall x R L t t', red_regular' R -> red_out R -> term t ->
+                         p_contextual_closure R t t' -> x \notin L ->
+                         p_contextual_closure R (pterm_abs (close t x)) (pterm_abs (close t' x)).
+Proof.
+ intros x R L t t' H0 H1 T H2 Fr.
+ apply p_abs_in with (L := L). intros z Fr'. 
+ apply red_out_pctx in H1. apply red_out_to_rename in H1.
+ apply H1 with (x := x). apply fv_close'. apply fv_close'.
+ replace (close t x ^ x) with t. replace (close t' x ^ x) with t'; trivial.
+ apply open_close_var. apply red_regular'_pctx in H0. apply H0 in H2. apply H2; trivial.
+ apply open_close_var; trivial. 
+Qed.
+
+Lemma trs_pctx_abs_in_close : forall x R L t t', red_regular' R -> red_out R -> term t ->
+                         trans_closure (p_contextual_closure R) t t' -> x \notin L ->
+                         trans_closure (p_contextual_closure R) (pterm_abs (close t x)) (pterm_abs (close t' x)).
+Proof.
+ intros x R L t t' H0 H1 T H Fr. induction H.
+ apply one_step_reduction. apply pctx_abs_in_close with (L := L); trivial.  
+  apply transitive_reduction with (u := pterm_abs (close u x)).
+ apply pctx_abs_in_close with (L := L); trivial.
+ apply IHtrans_closure. apply red_regular'_pctx in H0. 
+ apply H0 in H. apply H; trivial.
+Qed.
+
+
+Lemma trs_pctx_abs_in : forall R L t t', red_regular' R -> red_out R -> body t ->
+                       (forall x, x \notin L ->  trans_closure (p_contextual_closure R) (t ^ x) (t' ^ x)) ->
+                       trans_closure (p_contextual_closure R) (pterm_abs t) (pterm_abs t').
+Proof.
+ intros R L t t' H0 H1 B H2.  case var_fresh with (L := L \u (fv t) \u (fv t')). intros x Fr.
+ apply notin_union in Fr. destruct Fr. apply notin_union in H. destruct H.
+ assert (Q: trans_closure (p_contextual_closure R) (t ^ x) (t' ^ x)). apply H2; trivial. clear H2.
+ gen_eq t0 : (t ^ x). gen_eq t1 : (t' ^ x). intros Ht1 Ht0.
+ replace t with (close t0 x). replace t' with (close t1 x).
+ assert (T : term t0). rewrite Ht0. apply body_to_term; trivial.
+ clear Ht0 Ht1. induction Q.
+ apply one_step_reduction. apply pctx_abs_in_close with (L := L); trivial.
+ apply transitive_reduction with (u := pterm_abs (close u x)); trivial.
+ apply pctx_abs_in_close with (L := L); trivial. apply IHQ.
+ apply red_regular'_pctx in H0. apply H0 in H2. apply H2; trivial.
+ rewrite Ht1. rewrite <- close_open_term; trivial. 
+ rewrite Ht0. rewrite <- close_open_term; trivial.
+Qed.
+
+Lemma str_pctx_abs_in : forall R L t t', red_regular' R -> red_out R -> body t ->
+                       (forall x, x \notin L ->  star_closure (p_contextual_closure R) (t ^ x) (t' ^ x)) ->
+                       star_closure (p_contextual_closure R) (pterm_abs t) (pterm_abs t').
+Proof.
+ intros R L t t' H0 H1 B H2.  case var_fresh with (L := L \u (fv t) \u (fv t')). intros x Fr.
+ apply notin_union in Fr. destruct Fr. apply notin_union in H. destruct H.
+ assert (Q: star_closure (p_contextual_closure R) (t ^ x) (t' ^ x)). apply H2; trivial. clear H2.
+ gen_eq t0 : (t ^ x). gen_eq t1 : (t' ^ x). intros Ht1 Ht0.
+ replace t with (close t0 x). replace t' with (close t1 x).
+ assert (T : term t0). rewrite Ht0. apply body_to_term; trivial.
+ clear Ht0 Ht1. induction Q.
+ apply reflexive_reduction. apply star_trans_reduction. induction H2.
+ apply one_step_reduction. apply pctx_abs_in_close with (L := L); trivial.
+ apply transitive_reduction with (u := pterm_abs (close u x)); trivial.
+ apply pctx_abs_in_close with (L := L); trivial.
+ apply IHtrans_closure.
+ apply red_regular'_pctx in H0. apply H0 in H2. apply H2; trivial.
+ rewrite Ht1. rewrite <- close_open_term; trivial. 
+ rewrite Ht0. rewrite <- close_open_term; trivial.
+Qed.
+
+
+Lemma ctx_subst_left_close : forall x R L t t' u, red_regular R -> red_out R -> term u ->
+                         contextual_closure R t t' -> x \notin L ->
+                         contextual_closure R ((close t x)[u]) ((close t' x)[u]).
+Proof.
+ intros x R L t t' u H0 H1 T H2 Fr.
+ apply subst_left with (L := L); trivial. intros z Fr'. 
+ apply red_out_ctx in H1. apply red_out_to_rename in H1.
+ apply H1 with (x := x). apply fv_close'. apply fv_close'.
+ replace (close t x ^ x) with t. replace (close t' x ^ x) with t'; trivial.
+ apply open_close_var. apply red_regular_ctx in H0. apply H0 in H2. apply H2.
+ apply open_close_var. apply red_regular_ctx in H0. apply H0 in H2. apply H2.
+Qed.
+
+Lemma trs_ctx_subst_left : forall R L t t' u, red_regular R -> red_out R -> term u ->
+                       (forall x, x \notin L ->  trans_closure (contextual_closure R) (t ^ x) (t' ^ x)) ->
+                       trans_closure (contextual_closure R) (t[u]) (t'[u]).
+Proof.
+ intros R L t t' u H0 H1 T H2.  case var_fresh with (L := L \u (fv t) \u (fv t')). intros x Fr.
+ apply notin_union in Fr. destruct Fr. apply notin_union in H. destruct H.
+ assert (Q: trans_closure (contextual_closure R) (t ^ x) (t' ^ x)). apply H2; trivial. clear H2.
+ gen_eq t0 : (t ^ x). gen_eq t1 : (t' ^ x). intros Ht0 Ht1.
+ replace t with (close t0 x). replace t' with (close t1 x). clear Ht0 Ht1. induction Q.
+ apply one_step_reduction. apply ctx_subst_left_close with (L := L); trivial.
+ apply transitive_reduction with (u := (close u0 x)[u]); trivial.
+ apply ctx_subst_left_close with (L := L); trivial.
+ rewrite Ht0. rewrite <- close_open_term; trivial. 
+ rewrite Ht1. rewrite <- close_open_term; trivial.
+Qed.
+
+Lemma str_ctx_subst_left : forall R L t t' u, red_regular R -> red_out R -> term u ->
+                       (forall x, x \notin L ->  star_closure (contextual_closure R) (t ^ x) (t' ^ x)) ->
+                       star_closure (contextual_closure R) (t[u]) (t'[u]).
+Proof.
+ intros R L t t' u H0 H1 T H2.  case var_fresh with (L := L \u (fv t) \u (fv t')). intros x Fr.
+ apply notin_union in Fr. destruct Fr. apply notin_union in H. destruct H.
+ assert (Q: star_closure (contextual_closure R) (t ^ x) (t' ^ x)). apply H2; trivial. clear H2.
+ gen_eq t0 : (t ^ x). gen_eq t1 : (t' ^ x). intros Ht1 Ht0.
+ replace t with (close t0 x). replace t' with (close t1 x). clear Ht0 Ht1. destruct Q.
+ apply reflexive_reduction. apply star_trans_reduction. induction H2.
+ apply one_step_reduction. apply ctx_subst_left_close with (L := L); trivial.
+ apply transitive_reduction with (u := (close u0 x)[u]); trivial.
+ apply ctx_subst_left_close with (L := L); trivial.
+ rewrite Ht1. rewrite <- close_open_term; trivial. 
+ rewrite Ht0. rewrite <- close_open_term; trivial.
+Qed.
+
+
+Lemma pctx_subst_close : forall x R L t t' u u', red_regular' R -> red_out R -> term t -> term u ->
+                         p_contextual_closure R u u' ->
+                         p_contextual_closure R t t' -> x \notin L ->
+                         p_contextual_closure R ((close t x)[u]) ((close t' x)[u']).
+Proof.
+ intros x R L t t' u u' H0 H1 Tt Tu H2 H3 Fr.
+ apply p_subst with (L := L); trivial. intros z Fr'. 
+ apply red_out_pctx in H1. apply red_out_to_rename in H1.
+ apply H1 with (x := x). apply fv_close'. apply fv_close'.
+ replace (close t x ^ x) with t. replace (close t' x ^ x) with t'; trivial.
+ apply open_close_var. apply red_regular'_pctx in H0. apply H0 in H3. apply H3; trivial.
+ apply open_close_var; trivial. 
+Qed.
+
+Lemma trs_pctx_subst_close : forall x R L t t' u u', 
+                         red_regular' R -> red_out R -> (forall t0, R t0 t0) ->
+                         term t -> term u ->
+                         trans_closure (p_contextual_closure R) t t' -> 
+                         trans_closure (p_contextual_closure R) u u' -> x \notin L ->
+                         trans_closure (p_contextual_closure R) ((close t x)[u]) ((close t' x)[u']).
+Proof.
+ intros x R L t t' u u' H0 H1 H2 Tt Tu H3 H4 Fr. induction H3. induction H4.
+ apply one_step_reduction. apply pctx_subst_close with (L := L); trivial.  
+  apply transitive_reduction with (u := (close t x)[u]).
+ apply pctx_subst_close with (L := L); trivial. apply p_redex. apply H2. 
+ apply IHtrans_closure. apply red_regular'_pctx in H0. 
+ apply H0 in H3. apply H3; trivial.
+ apply transitive_reduction with (u := (close u0 x)[u]).
+ apply pctx_subst_close with (L := L); trivial. apply p_redex. apply H2.
+ apply IHtrans_closure. apply red_regular'_pctx in H0. 
+ apply H0 in H. apply H; trivial.
+Qed.
+
+
+Lemma trs_pctx_subst : forall R L t t' u u', red_regular' R -> red_out R -> (forall t0, R t0 t0) -> 
+                        body t -> term u ->
+                       (forall x, x \notin L ->  trans_closure (p_contextual_closure R) (t ^ x) (t' ^ x)) -> 
+                       trans_closure (p_contextual_closure R) u u' ->
+                       trans_closure (p_contextual_closure R) (t[u]) (t'[u']).
+Proof.
+ intros R L t t' u u' H0 H1 H2 B Tu H3 H4.  case var_fresh with (L := L \u (fv t) \u (fv t')). intros x Fr.
+ apply notin_union in Fr. destruct Fr. apply notin_union in H. destruct H.
+ assert (Q: trans_closure (p_contextual_closure R) (t ^ x) (t' ^ x)). apply H3; trivial. clear H3.
+ gen_eq t0 : (t ^ x). gen_eq t1 : (t' ^ x). intros Ht1 Ht0.
+ replace t with (close t0 x). replace t' with (close t1 x).
+ assert (T : term t0). rewrite Ht0. apply body_to_term; trivial.
+ clear Ht0 Ht1. induction Q. induction H4.
+ apply one_step_reduction. apply pctx_subst_close with (L := L); trivial.
+ apply transitive_reduction with (u := (close t0 x)[u]); trivial.
+ apply pctx_subst_close with (L := L); trivial. apply p_redex. apply H2. 
+ apply IHtrans_closure. apply red_regular'_pctx in H0. apply H0 in H4. apply H4; trivial.
+ apply transitive_reduction with (u := (close u0 x)[u]); trivial.
+ apply pctx_subst_close with (L := L); trivial. apply p_redex. apply H2. 
+ apply IHQ. apply red_regular'_pctx in H0. apply H0 in H3. apply H3; trivial.
+ rewrite Ht1. rewrite <- close_open_term; trivial. 
+ rewrite Ht0. rewrite <- close_open_term; trivial.
+Qed.
+
+Lemma str_pctx_subst : forall R L t t' u u', red_regular' R -> red_out R -> (forall t0, R t0 t0) -> 
+                        body t -> term u ->
+                       (forall x, x \notin L ->  star_closure (p_contextual_closure R) (t ^ x) (t' ^ x)) -> 
+                       star_closure (p_contextual_closure R) u u' ->
+                       star_closure (p_contextual_closure R) (t[u]) (t'[u']).
+Proof.
+ intros R L t t' u u' H0 H1 H2 B Tu H3 H4.  case var_fresh with (L := L \u (fv t) \u (fv t')). intros x Fr.
+ apply notin_union in Fr. destruct Fr. apply notin_union in H. destruct H.
+ assert (Q: star_closure (p_contextual_closure R) (t ^ x) (t' ^ x)). apply H3; trivial. clear H3.
+ gen_eq t0 : (t ^ x). gen_eq t1 : (t' ^ x). intros Ht1 Ht0.
+ replace t with (close t0 x). replace t' with (close t1 x).
+ assert (T : term t0). rewrite Ht0. apply body_to_term; trivial.
+ clear Ht0 Ht1. destruct H4. destruct Q. apply reflexive_reduction.
+ apply star_trans_reduction. induction H3.
+ apply one_step_reduction. apply pctx_subst_close with (L := L); trivial. apply p_redex. apply H2.
+ apply transitive_reduction with (u := (close u x)[t2]); trivial.
+ apply pctx_subst_close with (L := L); trivial. apply p_redex. apply H2. 
+ apply IHtrans_closure. apply red_regular'_pctx in H0. apply H0 in H3. apply H3; trivial.
+ destruct Q. apply star_trans_reduction. induction H3. apply one_step_reduction.
+ apply pctx_subst_close with (L := L); trivial. apply p_redex. apply H2.
+ apply transitive_reduction with (u := (close t0 x)[u]); trivial.
+ apply pctx_subst_close with (L := L); trivial. apply p_redex. apply H2. 
+ apply IHtrans_closure. apply red_regular'_pctx in H0. apply H0 in H3. apply H3; trivial.
+ apply star_trans_reduction. induction H3. induction H4.
+ apply one_step_reduction. apply pctx_subst_close with (L := L); trivial.
+ apply transitive_reduction with (u := (close u0 x)[t1]); trivial.
+ apply pctx_subst_close with (L := L); trivial. apply p_redex. apply H2. 
+ apply IHtrans_closure. apply red_regular'_pctx in H0. apply H0 in H4. apply H4; trivial.
+ apply transitive_reduction with (u := (close t0 x)[u]); trivial.
+ apply pctx_subst_close with (L := L); trivial. apply p_redex. apply H2. 
+ apply IHtrans_closure. apply red_regular'_pctx in H0. apply H0 in H3. apply H3; trivial.
+ rewrite Ht1. rewrite <- close_open_term; trivial. 
+ rewrite Ht0. rewrite <- close_open_term; trivial.
+Qed.
+*)
